add stuff

Abt.lean
@@ -1,103 +1,103 @@
 import Rec
+import Std.Data.List.Lemmas
 
-def Fin.zero : Fin (.succ n) :=
-  ⟨0, n.zero_lt_succ⟩
-
-def Fin.last : Fin (.succ n) :=
-  ⟨n, n.lt_succ_self⟩
-
-def Fin.castSucc : Fin n → Fin n.succ
-  | ⟨i, h⟩ => ⟨i, .step h⟩
+private def True.casesOn' {motive : True → Sort u} t (intro : motive intro) : motive t := intro
+@[csimp] theorem True.casesOn_eq' : @True.casesOn = @True.casesOn' := by
+  funext motive t intro
+  rfl
 
 def String.joinSep l sep := join (List.intersperse sep l)
 
-/-
-def Fin.cast (h' : k ≤ n) : Fin k → Fin n
-  | ⟨i, h⟩ => ⟨i, Nat.le_trans h h'⟩
+theorem Nat.le_trans_lt {n m k : Nat} (h₁ : n ≤ m) (h₂ : m < k) : n < k :=
+  Nat.le_trans (succ_le_succ h₁) h₂
 
-def Fin.cases {α : Fin (n + 1) → Sort u} (zero : α .zero) (succ : ∀ i, α (Fin.succ i)) : ∀ i, α i
-  | ⟨0, _⟩ => zero
-  | ⟨i + 1, h⟩ => succ ⟨i, Nat.pred_le_pred h⟩
+theorem Nat.le_of_le_add_right {n m k : Nat} (h : n + k ≤ m) : n ≤ m := by
+  induction k with
+  | zero => exact h
+  | succ k ih => exact ih (Nat.le_of_succ_le_succ h.step)
 
-def Fin.revCases {α : Fin (n + 1) → Sort u} (last : α .last) (castSucc : ∀ i, α (Fin.castSucc i)) : ∀ i, α i
-  | ⟨i, h⟩ =>
-    if h' : i = n
-    then by simp [h']; exact last
-    else castSucc ⟨i, Nat.lt_of_le_of_ne (Nat.pred_le_pred h) h'⟩
+theorem Nat.le_of_le_add_left {n m k : Nat} (h : k + n ≤ m) : n ≤ m := by
+  rw [Nat.add_comm] at h
+  exact Nat.le_of_le_add_right h
 
-namespace FinTuple
+theorem Nat.lt_of_lt_add_left {n m k : Nat} (h : k + n ≤ m) : n ≤ m := Nat.le_of_le_add_left h
 
-def foldr' {α : Fin n → Sort u} (f : ∀ {i}, Nat → α i → β → β) (y : β) (xs : ∀ i, α i) : β :=
-  foldr (λ x (y, k) => (f k x y, k + 1)) (y, 0) xs |>.1
+theorem Nat.lt_of_lt_add_right {n m k : Nat} (h : n + k < m) : n < m := by
+  rw [Nat.add_comm] at h
+  exact Nat.lt_of_lt_add_left h
 
-def dfoldr {α : Fin n → Sort u} {β : Fin (n + 1) → Sort v} (f : ∀ {i}, α i → β i.succ → β i.castSucc) (y : β .last) (xs : ∀ i, α i) : β .zero :=
-  match n with
-  | 0 => y
-  | _ + 1 => f (xs .zero) (dfoldr (β := β ∘ .succ) f y (xs ·.succ))
+theorem lt_of_compare_lt {x y : α} [LT α] [Decidable (x < y)] [DecidableEq α] (h : compareOfLessAndEq x y = .lt) : x < y := by
+  unfold compareOfLessAndEq at h
+  split at h
+  . assumption
+  . split at h
+    . contradiction
+    . contradiction
 
-def dfoldl {α : Fin n → Sort u} {β : Fin (n + 1) → Sort v} (f : ∀ {i}, β i.castSucc → α i → β i.succ) (y : β .zero) (xs : ∀ i, α i) : β .last :=
-  match n with
-  | 0 => y
-  | _ + 1 => dfoldl (β := β ∘ .succ) (f ·) (f (i := .zero) y (xs .zero)) (xs ·.succ)
+theorem eq_of_compare_eq {x y : α} [LT α] [Decidable (x < y)] [DecidableEq α] (h : compareOfLessAndEq x y = .eq) : x = y := by
+  unfold compareOfLessAndEq at h
+  split at h
+  . contradiction
+  . split at h
+    . assumption
+    . contradiction
 
-def toStringAux : ∀ {n} {α : Fin n → Type u} [∀ i, ToString (α i)], Bool → (∀ i, α i) → String
-  | 0, _, _, _, _ => ""
-  | _ + 1, _, _, true, xs => toString (xs 0) ++ toStringAux false (xs ·.succ)
-  | _ + 1, _, _, false, xs => ", " ++ toString (xs 0) ++ toStringAux false (xs ·.succ)
+theorem gt_of_compare_gt {x y : Nat} (h : compare x y = .gt) : x > y := by
+  dsimp [compare, compareOfLessAndEq] at h
+  split at h
+  . contradiction
+  . split at h
+    . contradiction
+    . apply Nat.gt_of_not_le
+      intro h
+      cases Nat.eq_or_lt_of_le h
+      . contradiction
+      . contradiction
 
-instance {α : Fin n → Type u} [∀ i, ToString (α i)] : ToString (∀ i, α i) where
-  toString xs := "⟦" ++ toStringAux true xs ++ "⟧"
+theorem Nat.le_max₁ (x y : Nat) : x ≤ max x y := by
+  rw [Nat.max_def]
+  split
+  . assumption
+  . exact .refl
 
-macro "⟦" t:term,* "⟧'" : term => `(@Sigma.mk Nat ((_ : Fin ·) → _) _ ⟦$t,*⟧)
+theorem Nat.le_max₂ (x y : Nat) : y ≤ max x y := by
+  rw [Nat.max_def]
+  split
+  . exact .refl
+  . rename_i h
+    exact Nat.ge_of_not_lt (h ∘ Nat.le_of_lt)
 
-end FinTuple
--/
+inductive List.Suffix {α : Type u} : List α → List α → Prop
+  | refl : Suffix l l
+  | cons x : Suffix l₁ l₂ → Suffix l₁ (x :: l₂)
 
-namespace FinTuple
+theorem List.Suffix.nil : {l : List α} → Suffix [] l
+  | [] => .refl
+  | x :: _ => .cons x nil
 
-def nil {α : Fin 0 → Sort u} i : α i := nomatch i
+theorem List.Suffix.tail : Suffix (x :: l₁) l₂ → Suffix l₁ l₂
+  | refl => cons x refl
+  | cons y s => cons y <| tail s
 
-def cons {α : Fin (.succ n) → Sort u} (x : α .zero) (xs : ∀ i, α (.succ i)) : ∀ i, α i
-  | ⟨0, _⟩ => x
-  | ⟨i + 1, h⟩ => xs ⟨i, Nat.lt_of_succ_lt_succ h⟩
+theorem List.mem_of_mem_suffix (m : x ∈ l₁) : Suffix l₁ l₂ → x ∈ l₂
+  | .refl => m
+  | .cons y s => .tail y <| mem_of_mem_suffix m s
 
-scoped syntax "⟦" term,* "⟧" : term
+def List.recSuffix (l : List α) {motive : ∀ l', l'.Suffix l → Sort _}
+  (nil : motive [] .nil)
+  (cons : ∀ x xs h, motive xs h.tail → motive (x :: xs) h)
+: motive l .refl :=
+  match l with
+  | [] => nil
+  | x :: xs => cons x xs .refl (@recSuffix α xs (motive · <| .cons _ ·) nil (cons · · <| .cons _ ·))
 
-macro_rules
-  | `(⟦⟧)          => ``(nil)
-  | `(⟦$x⟧)        => ``(cons $x ⟦⟧)
-  | `(⟦$x, $xs,*⟧) => ``(cons $x ⟦$xs,*⟧)
-
-@[app_unexpander nil]
-protected def nilUnexpander : Lean.PrettyPrinter.Unexpander
-  | `($_:ident) => ``(⟦⟧)
-  | _           => throw ()
-
-@[app_unexpander cons]
-protected def consUnexpander : Lean.PrettyPrinter.Unexpander
-  | `($_ $x ⟦⟧)      => ``(⟦$x⟧)
-  | `($_ $x ⟦$xs,*⟧) => ``(⟦$x, $xs,*⟧)
-  | _                => throw ()
-
-def foldr {α : Fin n → Sort u} {β : Sort v} (f : ∀ {i}, α i → β → β) (y : β) (xs : ∀ i, α i) : β :=
-  match n with
-  | 0 => y
-  | _ + 1 => f (xs .zero) (foldr f y (xs ·.succ))
-
-def foldl {α : Fin n → Sort u} {β : Sort v} (f : ∀ {i}, β → α i → β) (y : β) (xs : ∀ i, α i) : β :=
-  match n with
-  | 0 => y
-  | _ + 1 => foldl f (f y (xs .zero)) (xs ·.succ)
-
-def toList : (Fin n → α) → List α :=
-  foldr .cons .nil
-
-end FinTuple
-
-variable {α : Type u} (β : α → Sort v) in
-inductive DList : List α → Sort _
+variable {τ : Type u} (α : τ → Sort v) in
+inductive DList : List τ → Sort _
   | nil : DList []
-  | cons : β a → DList as → DList (a :: as)
+  | cons : α t → DList ts → DList (t :: ts)
+
+#compile List
+#compile DList
 
 namespace DList
 
@@ -118,415 +118,723 @@ protected def consUnexpander : Lean.PrettyPrinter.Unexpander
   | `($_ $x ⟦$xs,*⟧) => ``(⟦$x, $xs,*⟧)
   | _                => throw ()
 
-variable {α : Type u} {β₁ : α → Type v₁} {β₂ : α → Type v₂} (f : ∀ {a}, β₁ a → β₂ a) in
-def map : DList β₁ as → DList β₂ as
+variable {τ : Type u} {α : τ → Sort v} {β : Sort w}
+
+def recSuffix
+  {ts : List τ} {motive : ∀ ts', ts'.Suffix ts → DList α ts' → Sort w}
+  (nil : motive [] .nil nil)
+  (cons : ∀ {t ts'} x xs h, motive ts' h.tail xs → motive (t :: ts') h (cons x xs))
+  (xs : DList α ts)
+: motive ts .refl xs :=
+  match ts, xs with
+  | _, .nil => nil
+  | _, .cons x xs => cons x xs .refl (@recSuffix _ (motive · <| .cons _ ·) nil (cons · · <| .cons _ ·) xs)
+
+/-
+variable
+  {motive : ∀ ts, DList α ts → Sort w}
+  (nil : motive [] nil) in
+@[simp]
+def recMem {ts : List τ} (cons : ∀ {t ts'} x xs, t ∈ ts → motive ts' xs → motive (t :: ts') (cons x xs)) : ∀ xs, motive ts xs
+  | .nil => nil
+  | .cons x xs => cons x xs (.head _) (recMem (cons · · <| .tail _ ·) xs)
+-/
+
+variable (f : ∀ t, α t) in
+@[simp]
+def mk : ∀ ts, DList α ts
+  | [] => nil
+  | t :: ts => cons (f t) (mk ts)
+
+@[simp]
+def mkMem : ∀ ts, (∀ {t}, t ∈ ts → α t) → DList α ts
+  | [], _ => nil
+  | t :: ts, f => cons (f (.head ts)) (mkMem ts λ h => f (.tail t h))
+
+variable {α' : τ → Sort v'} (f : ∀ {t}, α t → α' t) in
+@[simp]
+def map : DList α ts → DList α' ts
   | nil => nil
   | cons x xs => cons (f x) (map xs)
 
-variable {α : Type u} {β : α → Sort v} {γ : Sort w} (f : ∀ {a}, β a → γ → γ) (y : γ) in
-def foldr : DList β as → γ
+variable {α' : τ → Sort v'} in
+@[simp]
+def mapMem (f : ∀ {t}, t ∈ ts → α t → α' t) : DList α ts → DList α' ts
+  | nil => nil
+  | cons x xs => cons (f (.head _) x) (mapMem (λ h => f (.tail _ h)) xs)
+
+/-
+variable {α₁ : τ → Sort v₁} {α₂ : τ → Sort v₂} in
+@[simp]
+theorem map_map (f : ∀ {t}, α₁ t → α₂ t) (g : ∀ {t}, α t → α₁ t) {ts} : ∀ xs, @map τ α₁ α₂ @f ts (@map τ α α₁ @g ts xs) = @map τ α α₂ (f <| g ·) ts xs
+  | nil => rfl
+  | cons .. => congrArg _ (map_map ..)
+-/
+
+/-
+variable {α₁ : τ → Sort v₁} {α₂ : τ → Sort v₂} in
+@[simp]
+theorem map_mapMem (f : ∀ {t}, α₁ t → α₂ t) {ts} (g : ∀ {t}, t ∈ ts → α t → α₁ t) (xs : DList α ts) : @map τ α₁ α₂ @f ts (@mapMem τ α α₁ ts @g xs) = @mapMem τ α α₂ ts (f <| g · ·) xs :=
+  match ts, xs with
+  | _, nil => rfl
+  | _, cons .. => congrArg _ (map_mapMem ..)
+-/
+
+variable (f : ∀ {t}, α t → β → β) (y : β) in
+@[simp]
+def foldr : DList α ts → β
   | nil => y
   | cons x xs => f x (foldr xs)
 
-def toList : DList (λ _ => α) as → List α :=
-  foldr .cons .nil
+variable (f : ∀ {t}, β → α t → β) in
+@[simp]
+def foldl (y : β) {ts} : DList α ts → β
+  | nil => y
+  | cons x xs => foldl (f y x) xs
+
+variable {α : Type v} in
+@[simp]
+def toList {ts : List τ} : DList (λ _ => α) ts → List α
+  | nil => []
+  | cons x xs => x :: toList xs
+
+instance instToString {α : τ → Type v} [∀ t, ToString (α t)] {ts} : ToString (DList α ts) where
+  toString xs := xs.map toString |>.toList.toString
+
+instance instInhabited [∀ t, Inhabited (α t)] : Inhabited (DList α ts) where
+  default := default' ts
+where
+  default'
+    | [] => .nil
+    | _ :: ts => .cons default (default' ts)
 
 end DList
 
-structure Var (s : α) where
+structure Var {S : Sort u} (s : S) where
   x : Nat
+  deriving Inhabited
 
-instance : DecidableEq (Var s)
+namespace Var
+
+variable {S : Sort u} {s : S}
+
+instance instDecidableEq : DecidableEq (Var s)
   | ⟨x⟩, ⟨y⟩ =>
     if h : x = y
     then isTrue (congrArg Var.mk h)
     else isFalse (h ∘ congrArg Var.x)
 
-instance : OfNat (Var s) n := ⟨⟨n⟩⟩
+instance instOfNat : OfNat (Var s) n := ⟨⟨n⟩⟩
 
-protected partial def Var.toString : Var s → String
-  | ⟨x⟩ => ⟨f x []⟩
-where f x s :=
-  let s := Char.ofNat ('a'.toNat + x % 26) :: s
-  match x / 26 with
-  | 0 => s
-  | q + 1 => f q s
+protected def toString : Var s → String
+  | ⟨x⟩ => ⟨toString x []⟩
+where
+  toString x l :=
+    let l := Char.ofNat ('a'.toNat + x % 26) :: l
+    match h : x / 26 with
+    | 0 => l
+    | q + 1 =>
+      have := h ▸ Nat.div_le_self ..
+      toString q l
 
-instance : ToString (Var s) := ⟨Var.toString⟩
+instance instToString : ToString (Var s) := ⟨Var.toString⟩
 
-instance : Coe String (Var s) where
-  coe s := ⟨s.foldl (λ x c => (x + 1) * 26 + (c.toNat - 'a'.toNat).min 25) 0 - 26 ^ s.length⟩
+def ofString : String → Var s
+  | ⟨l⟩ =>
+    ⟨l.foldl (λ x c => (x + 1) * 26 + (c.toNat - 'a'.toNat).min 25) 0 - 26 ^ l.length⟩
+
+instance instCoeString : Coe String (Var s) := ⟨ofString⟩
+
+end Var
+abbrev isBound (O : List (List S × S) → S → Type) s :=
+  ∃ (si t : _) (_ : O si t) (b : _), b ∈ si.map Prod.fst ∧ s ∈ b
+
+variable {S : Type} (O : List (List S × S) → S → Type) in
+inductive Abt : S → Type
+  | bvar s (n : Nat) : Abt s
+  | var (v : isBound O s) (x : Var s) : Abt s
+  | op (o : O si s) (ai : DList (Abt ·.2) si) : Abt s
+
+#compile mutual Abt
+
+namespace Abt
+
+variable {S : Type} {O : List (List S × S) → S → Type}
+
+instance instInhabited : Inhabited (Abt O s) := ⟨.bvar s 0⟩
+
+def subst [DecidableEq S] {s} (a : Abt O s) (x : Var s) : ∀ {t}, Abt O t → Abt O t := @rec S O (λ s _ => Abt O s) (λ si _ => DList (Abt O ·.2) si)
+  bvar
+  (λ {t} v y => if h : t = s then if h ▸ y = x then h ▸ a else var v y else var v y)
+  (λ o _ => op o)
+  DList.nil
+  (λ _ _ => DList.cons (τ := _ × S) (α := (Abt O ·.2)))
+
+variable [DecidableEq S]
+
+variable (s : S) in
+protected def bindCount : List S → Nat
+  | [] => 0
+  | t :: ts => Abt.bindCount ts + if s = t then 1 else 0
+
+def bind {s : S} (x : Var s) : ∀ {t}, Abt O t → Nat → Abt O t := @rec S O (λ s _ => Nat → Abt O s) (λ si _ => Nat → DList (Abt O ·.2) si)
+  (λ t m _ => bvar t m)
+  (λ {t} v y n => if h : t = s then if h ▸ y = x then bvar t n else var v y else var v y)
+  (λ o _ ai' n => op o (ai' n))
+  (λ _ => .nil)
+  (λ {b _} _ _ f fi n => .cons (f (n + Abt.bindCount s b.1)) (fi n))
+
+def unbind (a : Abt O s) : ∀ {t}, Abt O t → Nat → Abt O t := @rec S O (λ s _ => Nat → Abt O s) (λ si _ => Nat → DList (Abt O ·.2) si)
+  (λ t m n => if h : t = s then match compare m n with | .lt => bvar t m | .eq => h ▸ a | .gt => bvar t (m - 1) else bvar t m)
+  (λ v x _ => var v x)
+  (λ o _ ai' n => op o (ai' n))
+  (λ _ => .nil)
+  (λ {b _} _ _ f fi n => .cons (f (n + Abt.bindCount s b.1)) (fi n))
+
+def unbind' (a : Abt O s) : ∀ {si : List (List S × S)}, DList (Abt O ·.2) si → Nat → DList (Abt O ·.2) si := @rec_1 S O (λ s _ => Nat → Abt O s) (λ si _ => Nat → DList (Abt O ·.2) si)
+  (λ t m n => if h : t = s then match compare m n with | .lt => bvar t m | .eq => h ▸ a | .gt => bvar t (m - 1) else bvar t m)
+  (λ v x _ => var v x)
+  (λ o _ ai' n => op o (ai' n))
+  (λ _ => .nil)
+  (λ {b _} _ _ f fi n => .cons (f (n + Abt.bindCount s b.1)) (fi n))
+
+def wellFormed : ∀ {s}, Abt O s → (_ : S → Nat := λ _ => 0) → Prop := @rec S O _ (λ _ _ => _ → _)
+  (λ s n N => n < N s)
+  (λ _ _ _ => True)
+  (λ _ _ hai N => hai N)
+  (λ _ => True)
+  (λ {b _} _ _ ha hai N => ha (λ s => N s + Abt.bindCount s b.1) ∧ hai N)
+
+def wellFormed' : {si : List (List S × S)} → DList (Abt O ·.2) si → (_ : S → Nat := λ _ => 0) → Prop := @rec_1 S O (λ _ _ => _ → _) _
+  (λ s n N => n < N s)
+  (λ _ _ _ => True)
+  (λ _ _ (hai : _ → _) N => hai N)
+  (λ _ => True)
+  (λ {b _} _ _ ha hai N => ha (λ s => N s + Abt.bindCount s b.1) ∧ hai N)
+
+@[simp]
+theorem wellFormed_op {o : O si s} : wellFormed (.op o ai) N = wellFormed' ai N := rfl
+
+@[simp]
+theorem wellFormed'_cons {b : _ × _} {a : Abt O b.2} : wellFormed' (.cons a ai) N = (wellFormed a (λ s => N s + Abt.bindCount s b.1) ∧ wellFormed' ai N) := rfl
+
+def wellFormed_zip {si : List (List S × S)} : (ai : DList (Abt O ·.2) si) → wellFormed' ai N → DList (λ b => { x : Abt O b.2 // x.wellFormed λ s => N s + Abt.bindCount s b.1 }) si
+  | .nil, _ => .nil
+  | .cons a ai, wf => .cons ⟨a, wf.1⟩ (wellFormed_zip ai wf.2)
+
+theorem wellFormed_weaken (h : ∀ s, N s ≤ N' s) {s} : {a : Abt O s} → wellFormed a N → wellFormed a N'
+  | bvar s _, wf => Nat.le_trans wf (h s)
+  | var .., wf => wf
+  | op _ ai, wf => weaken ai wf
+where
+  weaken {_}
+  | .nil, wf => wf
+  | .cons _ ai, wf => ⟨wellFormed_weaken (λ s => Nat.add_le_add_right (h s) _) wf.1, weaken ai wf.2⟩
+
+theorem wellFormed_bind (x : Var s) {n} (h : n < N s) {t} : {a : Abt O t} → wellFormed a N → wellFormed (bind x a n) N
+  | bvar .., wf => wf
+  | var .., wf => by
+    dsimp [bind]
+    split
+    . rename_i h'
+      split
+      . exact h' ▸ h
+      . exact wf
+    . exact wf
+  | op _ ai, wf => bind' ai wf
+where
+  bind' {_}
+  | .nil, wf => wf
+  | .cons _ ai, wf => ⟨wellFormed_bind x (Nat.add_lt_add_right h _) wf.1, bind' ai wf.2⟩
+
+theorem wellFormed_unbind {a : Abt O s} (h : wellFormed a N) {n} (h' : n ≤ N s) : {a' : Abt O t} → wellFormed a' (λ u => if u = s then N u + 1 else N u) → wellFormed (unbind a a' n) N
+  | bvar _ m, wf => by
+    dsimp [unbind]
+    split <;> rename_i h
+    . cases h
+      split
+      . rename_i h''
+        exact Nat.le_trans (lt_of_compare_lt h'' :) h'
+      . exact h
+      . cases m with
+        | zero =>
+          rename_i h
+          dsimp [compare, compareOfLessAndEq] at h
+          split at h
+          . cases h
+          . split at h
+            . cases h
+            . cases Nat.eq_or_lt_of_le (Nat.zero_le n)
+              . contradiction
+              . contradiction
+        | succ m =>
+          simp [wellFormed] at wf
+          exact Nat.lt_of_succ_lt_succ wf
+    . simp [wellFormed, h] at wf
+      exact wf
+  | var .., wf => wf
+  | op _ ai, wf => unbind' ai wf
+where
+  unbind' {_}
+  | .nil, wf => wf
+  | .cons _ ai, wf => ⟨by
+    apply wellFormed_unbind _ (Nat.add_le_add_right h' _)
+    . have : wellFormed _ _ := wf.1
+      dsimp at this
+      suffices _ = _ by
+        apply (congrArg _ this).mp
+        assumption
+      funext u
+      split
+      . apply Nat.add_right_comm
+      . rfl
+    . exact wellFormed_weaken (λ _ => Nat.le_add_right ..) h,
+  unbind' ai wf.2⟩
+
+theorem wellFormed_subst {a : Abt O s} (wfa : wellFormed a) (x : Var s) : {b : Abt O t} → wellFormed b N → wellFormed (subst a x b) N
+  | bvar .., wfb => wfb
+  | var .., wfb => by
+    dsimp [subst]
+    split
+    next h =>
+      cases h
+      dsimp
+      split
+      . exact wellFormed_weaken (λ _ => Nat.zero_le _) wfa
+      . exact wfb
+    . exact wfb
+  | op _ ai, wfb => subst' ai wfb
+where
+  subst' {_}
+  | .nil, wfb => wfb
+  | .cons b ai, wfb => ⟨wellFormed_subst wfa x wfb.1, subst' ai wfb.2⟩
+
+def freeIn {s : S} (x : Var s) : ∀ {t}, Abt O t → Prop := @rec S O _ _
+  (λ _ _ => True)
+  (λ {t} _ y => (h : t = s) → h ▸ y ≠ x)
+  (λ _ _ hai => hai)
+  True
+  (λ _ _ ha hai => ha ∧ hai)
+
+def freeIn' {s : S} (x : Var s) : {si : List (List S × S)} → DList (Abt O ·.2) si → Prop := @rec_1 S O (λ _ _ => _) _
+  (λ _ _ => True)
+  (λ {t} _ y => (h : t = s) → h ▸ y ≠ x)
+  (λ _ _ hai => hai)
+  True
+  (λ _ _ ha hai => ha ∧ hai)
+
+@[simp]
+theorem freeIn_op {s : S} : freeIn x (.op o ai) = freeIn' x ai := rfl
+
+theorem bind_unbind (v : isBound O s) (x : Var s) n (h : n + 1 = N s) : (a : Abt O t) → wellFormed a N → freeIn x a → bind x (unbind (var v x) a n) n = a
+  | bvar t m, wf, _ => by
+    dsimp [wellFormed] at wf
+    dsimp [unbind]
+    split
+    . rename_i h
+      cases h
+      split
+      . rfl
+      . rename_i h
+        have := eq_of_compare_eq h
+        simp [bind, this]
+      . rw [← h] at wf
+        rename_i h
+        cases Nat.not_succ_le_self _ (Nat.le_trans wf (gt_of_compare_gt h))
+    . rfl
+  | var _ y, _, hx => by
+    dsimp [unbind, bind]
+    split
+    . rename_i h
+      cases h
+      split
+      . rename_i h
+        cases hx rfl h
+      . rfl
+    . rfl
+  | op o ai, wf, hx => congrArg (op o) <| thm' ai wf hx
+where
+  thm' {_}
+  | .nil, _, _ => rfl
+  | .cons a ai, wf, hx => by
+    apply congr (congrArg _ _) (thm' ai wf.2 hx.2)
+    apply bind_unbind v x (n + Abt.bindCount s _) _ a wf.1 hx.1
+    rw [Nat.add_right_comm]
+    exact congrArg (· + _) h
+
+def op' (o : O si s) (ai : DList (λ b => DList Var b.1 × Abt O b.2) si) : Abt O s :=
+  .op o <| ai.map λ a => a.1.foldr (β := _ × _) (λ {t} x (a, n) => (bind x a (n t), λ u => if u = t then n u + 1 else n u)) (a.2, λ _ : S => 0) |>.1
+
+def free (s : S) : ∀ {t}, Abt O t → Var s := @rec S O _ _
+  (λ _ _ => ⟨0⟩)
+  (λ {t} _ x => if t = s then ⟨x.1 + 1⟩ else ⟨0⟩)
+  (λ _ _ hai => hai)
+  ⟨0⟩
+  (λ _ _ x y => ⟨max x.1 y.1⟩)
+
+def free' (s : S) : {si : List (List S × S)} → DList (Abt O ·.2) si → Var s := @rec_1 S O (λ _ _ => _) _
+  (λ _ _ => ⟨0⟩)
+  (λ {t} _ x => if t = s then ⟨x.1 + 1⟩ else ⟨0⟩)
+  (λ _ _ hai => hai)
+  ⟨0⟩
+  (λ _ _ x y => ⟨max x.1 y.1⟩)
+
+@[simp]
+theorem free_op {s : S} : free s (.op o ai) = free' s ai := rfl
+
+theorem freeIn_free' (s : S) (x : Var s) : (a : Abt O t) → (free s a).1 ≤ x.1 → freeIn x a
+  | bvar .., _ => trivial
+  | var .., hx => by
+    intro h
+    cases h
+    dsimp [free] at hx
+    rw [if_pos rfl] at hx
+    intro h
+    cases h
+    apply Nat.not_succ_le_self
+    exact hx
+  | op _ ai, hx => h ai hx
+where
+  h {si : List (List S × S)} : (ai : DList (Abt O <| Prod.snd ·) si) → (free' s ai).1 ≤ x.1 → freeIn' x ai
+  | .nil, _ => trivial
+  | .cons a ai, hx => ⟨freeIn_free' s x a <| Nat.le_trans (Nat.le_max₁ ..) hx, h ai <| Nat.le_trans (Nat.le_max₂ ..) hx⟩
+
+theorem freeIn_free (s : S) (a : Abt O t) : freeIn (free s a) a := freeIn_free' s _ a .refl
+
+def unop' : ∀ {si : List S}, DList (isBound O) si → Abt O s → DList Var si × Abt O s
+  | [], _ => (.nil, ·)
+  | s' :: si, .cons v vs => λ a =>
+    let x := a.free s'
+    let (xs, a) := unop' vs (unbind (var v x) a (Abt.bindCount s' si))
+    (.cons x xs, a)
+
+def unop (o : O si s) : DList (Abt O ·.2) si → DList (λ b => DList Var b.1 × Abt O b.2) si :=
+  .mapMem (unop' <| .mkMem _ λ h => ⟨si, s, o, _, List.mem_map_of_mem Prod.fst ·, h⟩)
+
+protected partial def toString [∀ si s, ToString (O si s)] {s} : Abt O s → String
+  | .bvar _ x => "#" ++ toString x
+  | .var _ x => x.toString
+  | .op o .nil => toString o
+  | .op o ai =>
+    toString o ++ "(" ++ .joinSep (unop o ai |>.map @λ
+      | (_, _), (.nil, a) => a.toString
+      | (_, _), (xi, a) => .joinSep (xi.map Var.toString).toList ", " ++ ". " ++ a.toString
+    ).toList "; " ++ ")"
+
+instance instToString [∀ si s, ToString (O si s)] {s} : ToString (Abt O s) := ⟨Abt.toString⟩
+
+instance instDecidableEq [∀ si s, DecidableEq (O si s)] : DecidableEq (Abt O s)
+  | .bvar _ n, .bvar _ m => if h : n = m then h ▸ isTrue rfl else isFalse (h ∘ bvar.inj)
+  | .var _ x, .var _ y => if h : x = y then h ▸ isTrue rfl else isFalse (h ∘ var.inj)
+  | .op (si := si) o ai, .op (si := si') o' ai' =>
+    if h : si = si'
+    then by cases h; exact
+      if h : o = o'
+      then h ▸
+        match op ai ai' with
+        | isTrue h => h ▸ isTrue rfl
+        | isFalse h => isFalse (h ∘ eq_of_heq ∘ And.right ∘ And.right ∘ op.inj)
+      else isFalse (h ∘ eq_of_heq ∘ And.left ∘ And.right ∘ op.inj)
+    else isFalse (h ∘ And.left ∘ op.inj)
+  | .bvar .., .var .. => isFalse (nomatch ·)
+  | .bvar .., .op .. => isFalse (nomatch ·)
+  | .var .., .bvar .. => isFalse (nomatch ·)
+  | .var .., .op .. => isFalse (nomatch ·)
+  | .op .., .bvar .. => isFalse (nomatch ·)
+  | .op .., .var .. => isFalse (nomatch ·)
+where
+  op {si : List (List S × S)} : DecidableEq (DList (Abt O ·.2) si)
+    | .nil, .nil => isTrue rfl
+    | .cons a ai, .cons a' ai' =>
+      match instDecidableEq a a' with
+      | isTrue h => h ▸
+        match op ai ai' with
+        | isTrue h => h ▸ isTrue rfl
+        | isFalse h => isFalse (h ∘ And.right ∘ DList.cons.inj)
+      | isFalse h => isFalse (h ∘ And.left ∘ DList.cons.inj)
+
+variable (Γ : ∀ {s : S}, Var s → Prop)
+
+def closed : ∀ {s}, Abt O s → Prop := @rec S O _ _
+  (λ _ _ => True)
+  (λ _ => Γ)
+  (λ _ _ hai => hai)
+  True
+  (λ _ _ => And)
+
+def closed' : ∀ {si : List (List S × S)}, DList (Abt O ·.2) si → Prop := @rec_1 S O (λ _ _ => _) _
+  (λ _ _ => True)
+  (λ _ => Γ)
+  (λ _ _ hai => hai)
+  True
+  (λ _ _ ha hai => ha ∧ hai)
+
+instance [∀ {s} (x : Var s), Decidable (Γ x)] : ∀ {s}, (a : Abt O s) → Decidable (closed Γ a) := @rec S O _ (λ _ ai => Decidable (closed' Γ ai))
+  (λ _ _ => isTrue trivial)
+  (λ _ _ => inferInstanceAs <| Decidable (Γ _))
+  (λ _ _ hai => hai)
+  (isTrue trivial)
+  (λ _ _ ha hai => match ha with | isFalse ha => isFalse (λ ⟨ha', _⟩ => ha ha') | isTrue ha => match hai with | isFalse hai => isFalse (λ ⟨_, hai'⟩ => hai hai') | isTrue hai => isTrue ⟨ha, hai⟩)
+
+theorem closed_unbind {a : Abt O s} (h : closed Γ a) : {a' : Abt O t} → closed Γ a' → closed Γ (unbind a a' n)
+  | bvar _ m, c => by
+    dsimp [unbind]
+    split <;> rename_i h
+    . cases h
+      split
+      . exact c
+      . exact h
+      . cases m with
+        | zero =>
+          rename_i h
+          dsimp [compare, compareOfLessAndEq] at h
+          split at h
+          . cases h
+          . split at h
+            . cases h
+            . cases Nat.eq_or_lt_of_le (Nat.zero_le n)
+              . contradiction
+              . contradiction
+        | succ m => exact c
+    . exact c
+  | var .., c => c
+  | op _ ai, c => unbind' ai c
+where
+  unbind' {_}
+  | .nil, c => c
+  | .cons _ ai, c => ⟨closed_unbind h c.1, unbind' ai c.2⟩
+
+theorem closed_subst {a : Abt O s} (ca : closed Γ a) (x : Var s) : {b : Abt O t} → closed Γ b → closed Γ (subst a x b)
+  | bvar .., cb => cb
+  | var .., cb => by
+    dsimp [subst]
+    split
+    next h =>
+      cases h
+      dsimp
+      split
+      . exact ca
+      . exact cb
+    . exact cb
+  | op _ ai, cb => subst' ai cb
+where
+  subst' {_}
+  | .nil, cb => cb
+  | .cons b ai, cb => ⟨closed_subst ca x cb.1, subst' ai cb.2⟩
+
+def sizeOf : ∀ {s}, Abt O s → Nat := @rec S O _ _
+  (λ _ _ => 1)
+  (λ _ _ => 1)
+  (λ _ _ hai => hai + 1)
+  0
+  (λ _ _ ha hai => ha + hai)
+
+def sizeOf' : ∀ {si : List (List S × S)}, DList (Abt O ·.2) si → Nat := @rec_1 S O (λ _ _ => _) _
+  (λ _ _ => 1)
+  (λ _ _ => 1)
+  (λ _ _ hai => hai + 1)
+  0
+  (λ _ _ ha hai => ha + hai)
+
+theorem sizeOf_unbind {a : Abt O s} (h : sizeOf a = 1) : (a' : Abt O t) → sizeOf (unbind a a' n) = sizeOf a'
+  | bvar .. => by
+    dsimp [unbind]
+    split
+    . split
+      . rfl
+      . rename_i h _ _
+        cases h
+        exact h
+      . rfl
+    . rfl
+  | var .. => rfl
+  | op _ ai => congrArg Nat.succ (f ai)
+where
+  f {si} : (ai : DList _ si) → _
+    | .nil => rfl
+    | .cons a' ai => by apply congr (congrArg Nat.add (sizeOf_unbind h a')) (f ai)
+
+end Abt
+
+def WfAbt (O : _ → S → _) [DecidableEq S] s := { a : Abt O s // a.wellFormed }
+
+namespace WfAbt
+
+variable {S : Type} {O : List (List S × S) → S → Type} [DecidableEq S]
+
+instance instToString [ToString (Abt O s)] : ToString (WfAbt O s) where
+  toString a := toString a.1
+
+instance instDecidableEq [∀ si s, DecidableEq (O si s)] : DecidableEq (WfAbt O s)
+  | ⟨x, _⟩, ⟨y, _⟩ => if h : x = y then isTrue (Subtype.eq h) else isFalse (h ∘ Subtype.mk.inj)
+
+def var (v : isBound O s) (x : Var s) : WfAbt O s := ⟨.var v x, trivial⟩
+
+def op (o : O si s) (ai : DList (WfAbt O ·.2) si) : WfAbt O s := ⟨.op o <| ai.map Subtype.val, by
+  dsimp [Abt.wellFormed]
+  clear o
+  induction ai with
+  | nil => trivial
+  | cons a ai hai => exact ⟨Abt.wellFormed_weaken (λ _ => Nat.zero_le _) a.2, hai⟩
+⟩
+
+def op' (o : O si s) (ai : DList (λ b => DList Var b.1 × WfAbt O b.2) si) : WfAbt O s := ⟨.op' o <| ai.map λ a => (a.1, a.2.1), by
+  dsimp [Abt.wellFormed, Abt.op']
+  clear o
+  induction ai with
+  | nil => trivial
+  | @cons b si a ai hai =>
+    apply And.intro _ hai
+    cases b with | _ si t =>
+    cases a with | _ xs a =>
+    dsimp at xs a ⊢
+    suffices let x : _ × (S → _) := DList.foldr ..; Abt.wellFormed x.1 _ ∧ (∀ s, x.2 s ≤ Abt.bindCount s si) by
+      exact this.1
+    induction xs with
+    | nil => exact ⟨Abt.wellFormed_weaken (λ _ => Nat.zero_le _) a.2, λ _ => .refl⟩
+    | @cons s si x xs hxs =>
+      dsimp [DList.foldr]
+      constructor
+      . apply Abt.wellFormed_bind
+        . apply Nat.le_trans_lt (hxs.2 s)
+          simp [Abt.bindCount]
+        . exact Abt.wellFormed_weaken (λ _ => Nat.add_le_add_left (Nat.le_add_right ..) 0) hxs.1
+      . intro t
+        split
+        . rename_i h
+          cases h
+          apply Nat.le_trans_lt (hxs.2 s)
+          simp [Abt.bindCount]
+        . apply Nat.le_trans (hxs.2 t) (Nat.le_add_right ..)
+⟩
+
+def unop' : ∀ {si}, DList (isBound O) si → (a : Abt O s) → a.wellFormed (Abt.bindCount · si) → DList Var si × WfAbt O s
+  | [], _ => (.nil, ⟨·, ·⟩)
+  | s' :: si, .cons v vs => λ a wf =>
+    let x := a.free s'
+    let (xs, a) := unop' vs (Abt.unbind (.var v x) a (Abt.bindCount s' si)) <| Abt.wellFormed_unbind (by exact trivial) (by exact .refl) (by apply Eq.mp (congrArg _ _) wf; funext u; dsimp [Abt.bindCount]; split <;> rename_i h; simp [h]; simp [Ne.symm h])
+    (.cons x xs, a)
+
+def unop (o : O si₁ s) {si : List (List S × S)} (hsi : si.Suffix si₁) : (ai : DList (Abt O ·.2) si) → Abt.wellFormed' ai → DList (λ b => DList Var b.1 × WfAbt O b.2) si
+  | .nil, _ => .nil
+  | .cons a ai, wf => .cons (unop' (.mkMem _ (⟨si₁, s, o, _, List.mem_map_of_mem _ (List.mem_of_mem_suffix (.head _) hsi), ·⟩)) a (by simp at wf; exact wf.1)) (unop o hsi.tail ai wf.2)
+
+variable (O) in
+inductive View : S → Type
+  | var (v : isBound O s) (x : Var s) : View s
+  | op (o : O si s) (ai : DList (λ b => DList Var b.1 × WfAbt O b.2) si) : View s
+
+#compile WfAbt.View
+
+def out : WfAbt O s → View O s
+  | ⟨.var v x, _⟩ => .var v x
+  | ⟨.op o ai, h⟩ => .op o (unop o .refl ai h)
+
+def View.in : View O s → WfAbt O s
+  | var v x => .var v x
+  | op o ai => .op' o ai
+
+theorem in_out : (a : WfAbt O s) → View.in (out a) = a := by
+  intro ⟨a, wf⟩
+  cases a with
+  | bvar => cases wf
+  | var => rfl
+  | @op si _ o ai =>
+    dsimp at wf
+    apply Subtype.eq _
+    apply congrArg (Abt.op o)
+    dsimp [unop]
+    have := @DList.recSuffix (List S × S) (Abt O ·.2) si (λ si' hs ai => (wf : _) → (
+      DList.map (λ a => a.1.foldr (β := _ × _) (λ {t} x (a, n) => (Abt.bind x a (n t), λ u => if u = t then n u + 1 else n u)) (a.2, λ _ : S => 0) |>.1) <|
+        DList.map (λ a => (a.1, a.2.1)) <|
+          unop o hs ai wf
+    ) = ai) ?nil ?cons ai wf
+    exact this
+    case nil => intro; rfl
+    case cons =>
+      clear wf ai
+      intro si si' a ai' hs hai wf
+      apply congr (congrArg _ _) (hai wf.2)
+      have : Abt.wellFormed _ _ := wf.1
+      simp at this
+      show (DList.foldr _ ((unop' _ a this).2.1, _) (unop' _ a this).1).1 = a
+      clear hai wf ai'
+      rename _ => wf
+      cases si with | _ si s =>
+      dsimp at a wf ⊢
+      suffices DList.foldr .. = (a, (Abt.bindCount · si)) from congrArg Prod.fst this
+      have := @List.recSuffix _ si (λ si₁ hs' => ∀ a (wf : _), DList.foldr
+        (λ {t} x (a, n) => (Abt.bind x a (n t), λ u => if u = t then n u + 1 else n u))
+        (unop' (.mkMem si₁ λ h' => ⟨_, _, o, _, List.mem_map_of_mem Prod.fst (List.mem_of_mem_suffix (.head _) hs), List.mem_of_mem_suffix h' hs'⟩) a wf |>.2.1, λ _ : S => 0)
+        (unop' (.mkMem si₁ λ h' => ⟨_, _, o, _, List.mem_map_of_mem Prod.fst (List.mem_of_mem_suffix (.head _) hs), List.mem_of_mem_suffix h' hs'⟩) a wf).1
+      = (a, (Abt.bindCount · si₁))) ?nil ?cons a wf
+      exact this
+      case nil => intro _ _; rfl
+      case cons =>
+        intro s' si hs' hsi a wf
+        dsimp [unop']
+        specialize hsi (Abt.unbind (.var ⟨_, _, o, _, List.mem_map_of_mem Prod.fst (List.mem_of_mem_suffix (.head _) hs), List.mem_of_mem_suffix (.head _) hs'⟩ (a.free s')) a (Abt.bindCount s' si)) _
+        . apply Abt.wellFormed_unbind
+          . trivial
+          . simp
+          . apply Eq.mp (congrArg _ _) wf
+            funext u
+            split <;> rename_i h <;> simp [Abt.bindCount, h]
+        generalize hB : DList.foldr .. = B
+        have := hB.symm.trans hsi
+        clear hB hsi
+        clear hsi
+        cases this
+        congr
+        . apply Abt.bind_unbind _ _ _ _ a wf (Abt.freeIn_free _ _)
+          simp [Abt.bindCount]
+        . funext u
+          split <;> rename_i h <;> simp [Abt.bindCount, h]
+
+def subst (a : WfAbt O s) (x : Var s) (b : WfAbt O t) : WfAbt O t := ⟨.subst a.1 x b.1, Abt.wellFormed_subst a.2 x b.2⟩
+
+def View.sizeOf : View O s → Nat
+  | .var .. => 1
+  | .op _ ai => Abt.sizeOf' (ai.map (·.2.1)) + 1
+
+@[simp]
+theorem sizeOf_out : (a : WfAbt O s) → (out a).sizeOf = a.1.sizeOf
+  | ⟨.var .., _⟩ => rfl
+  | ⟨.op o ai, wf⟩ => by
+    apply congrArg Nat.succ
+    revert ai
+    apply DList.recSuffix (motive := λ si hsi ai => (wf : _) → Abt.sizeOf' ((unop o hsi ai wf).map (·.2.1)) = Abt.sizeOf' ai)
+    case nil => intro; rfl
+    case cons =>
+      intro si si' a ai hsi ih wf
+      apply congr (congrArg Nat.add _) (ih wf.2)
+      clear ih
+      have : Abt.wellFormed _ _ := wf.1
+      simp at this
+      show Abt.sizeOf (unop' _ a this).2.1 = Abt.sizeOf a
+      clear wf
+      rename _ => wf
+      cases si with | _ si s' =>
+      dsimp at wf ⊢
+      apply @List.rec _ (λ si => (vs : _) → (a : _ ) → (wf : Abt.wellFormed a (Abt.bindCount · si)) → Abt.sizeOf (unop' vs a wf).2.1 = Abt.sizeOf a) ?nil ?cons si (.mkMem _ (⟨_, s, o, _, List.mem_map_of_mem Prod.fst (List.mem_of_mem_suffix (.head si') hsi), ·⟩)) a wf
+      case nil => intro .nil _ _; rfl
+      case cons =>
+        intro s si ih (.cons v vs) a wf
+        dsimp [unop']
+        apply ih vs (Abt.unbind (.var v (a.free s)) a (Abt.bindCount s si)) _ |>.trans
+        apply Abt.sizeOf_unbind
+        rfl
+
+end WfAbt
 
 /-
-syntax "ast " ident " where " (ident (" | " ident term*)*)* : command
-macro_rules
-  | `(ast $l where $[$s $[| $o $[$a]*]*]*) => do
-    let is ← (s.zip (o.zip a)).mapM λ (s, (o, a)) =>
-      `(inductive $s)
-    `(namespace $l $(⟨Lean.mkNullNode is⟩) end $l)
-
-set_option trace.Elab.command true in
-ast Example where
+abt ExampleAbt
   Exp
-  | var Var
   | num "[" Nat "]"
   | plus "(" Exp "; " Exp ")"
   | times "(" Exp "; " Exp ")"
+  | let "(" Exp "; " Var Exp ". " Exp ")"
 -/
-
-namespace Example
-
-inductive Exp
-  | var : Var Exp → Exp
-  | num : Nat → Exp
-  | plus : Exp → Exp → Exp
-  | times : Exp → Exp → Exp
-
-instance : ToString Exp where
-  toString := toString
-where
-  toString
-  | .var x => x.toString
-  | .num n => s!"num[{n}]"
-  | .plus e₁ e₂ => s!"plus({toString e₁}; {toString e₂})"
-  | .times e₁ e₂ => s!"times({toString e₁}; {toString e₂})"
-
-namespace Exp
-
-variable (e : Exp) (x : Var Exp) in
-def substExp : Exp → Exp
-  | var y => if y = x then e else .var y
-  | num n => num n
-  | plus e₁ e₂ => plus (substExp e₁) (substExp e₂)
-  | times e₁ e₂ => times (substExp e₁) (substExp e₂)
-
-#eval plus (num 2) (times (num 3) (var 0))
-#eval substExp (num 2) 0 (plus (var 0) (var 1))
-
-end Exp
-
-end Example
-
-variable {S : Type} (O : List S → S → Type) in
-inductive Ast : S → Type
-  | var (x : Var s) : Ast s
-  | op (o : O si s) (ai : DList Ast si) : Ast s
-
-#compile mutual Ast
-
-namespace Ast
-
-def ndrec
-  {motive : S → Type u}
-  (var : ∀ {s}, Var s → motive s)
-  (op : ∀ {si s}, O si s → DList (Ast O) si → DList motive si → motive s)
-: ∀ {s}, Ast O s → motive s :=
-  @rec S O (λ s _ => motive s) (λ si _ => DList motive si) var op DList.nil λ _ _ => DList.cons
-
-def subst [DecidableEq S] {s : S} (a : Ast O s) (x : Var s) : Ast O t → Ast O t :=
-  ndrec
-    (λ {t} y => if h : t = s then if h ▸ y = x then h ▸ a else var y else var y)
-    (λ o _ ai' => op o ai')
-
-protected def toString [∀ si s, ToString (O si s)] : Ast O s → String :=
-  ndrec
-    (λ x => x.toString)
-    (λ | o, .nil, _ => toString o
-       | o, _, ai' => toString o ++ "(" ++ .joinSep ai'.toList "; " ++ ")")
-
-end Ast
-
-instance [∀ si s, ToString (O si s)] : ToString (Ast O s) := ⟨Ast.toString⟩
-
-variable {S : Type} (O : ∀ ⦃n⦄, (Fin n → S) → S → Type) in
-inductive Ast' : S → Type
-  | var (x : Var s) : Ast' s
-  | op (o : @O n si s) (ai : ∀ i, Ast' (si i)) : Ast' s
-
-namespace Ast'
-
-variable [DecidableEq S] {s : S} (a : Ast' O s) (x : Var s) in
-def subst : Ast' O t → Ast' O t
-  | var y => if h : t = s then if h ▸ y = x then h ▸ a else var y else var y
-  | op o ai => op o λ i => subst (ai i)
-
-protected def toString [∀ {n} si s, ToString (@O n si s)] : Ast' O s → String
-  | var x => x.toString
-  | op (n := 0) o _ => toString o
-  | op o ai => toString o ++ "(" ++ .joinSep (FinTuple.toList λ i => (ai i).toString) "; " ++ ")"
-
-end Ast'
-
-instance [∀ {n} si s, ToString (@O n si s)] : ToString (Ast' O s) := ⟨Ast'.toString⟩
-
-namespace ExampleAst
-
-open DList
-
-inductive S
-  | Exp
-deriving DecidableEq
-
-inductive O : List S → S → Type
-  | num : Nat → O [] .Exp
-  | plus : O [.Exp, .Exp] .Exp
-  | times : O [.Exp, .Exp] .Exp
-
-instance : ToString (O si s) where
-  toString
-  | .num n => s!"num[{n}]"
-  | .plus => "plus"
-  | .times => "times"
-
-abbrev Ast := _root_.Ast O
-
-abbrev Exp := Ast .Exp
-
-namespace Exp
-
-def var (x : Var S.Exp) : Exp := .var x
-def num (n : Nat) : Exp := .op (.num n) ⟦⟧
-def plus (a b : Exp) : Exp := .op .plus ⟦a, b⟧
-def times (a b : Exp) : Exp := .op .times ⟦a, b⟧
-
-#eval plus (num 2) (times (num 3) (var 0))
-#eval Ast.subst (num 2) 0 (plus (var 0) (var 1))
-
-end Exp
-
-end ExampleAst
-
-namespace ExampleAst'
-
-open FinTuple
-
-inductive S
-  | Exp
-deriving DecidableEq
-
-inductive O : ∀ ⦃n⦄, (Fin n → S) → S → Type
-  | num : Nat → O ⟦⟧ .Exp
-  | plus : O ⟦.Exp, .Exp⟧ .Exp
-  | times : O ⟦.Exp, .Exp⟧ .Exp
-
-instance : ToString (O si s) where
-  toString
-  | .num n => s!"num[{n}]"
-  | .plus => "plus"
-  | .times => "times"
-
-abbrev Ast := _root_.Ast' O
-
-abbrev Exp := Ast .Exp
-
-namespace Exp
-
-def var (x : Var S.Exp) : Exp := .var x
-def num (n : Nat) : Exp := .op (.num n) ⟦⟧
-def plus (a b : Exp) : Exp := .op .plus ⟦a, b⟧
-def times (a b : Exp) : Exp := .op .times ⟦a, b⟧
-
-#eval plus (num 2) (times (num 3) (var 0))
-#eval Ast'.subst (num 2) 0 (plus (var 0) (var 1))
-
-end Exp
-
-end ExampleAst'
-
-variable {S : Type} (O : List (List S × S) → S → Type) in
-inductive Abt₁ : S → Type
-  | bvar s (n : Nat) : Abt₁ s
-  | var (x : Var s) : Abt₁ s
-  | op (o : O si s) (ai : DList (Abt₁ ·.2) si) : Abt₁ s
-
-#compile mutual Abt₁
-
-namespace Abt₁
-
-def ndrec
-  {motive : S → Type u}
-  (bvar : ∀ s, Nat → motive s)
-  (var : ∀ {s}, Var s → motive s)
-  (op : ∀ {si s}, O si s → DList (Abt₁ O ·.2) si → DList (motive ·.2) si → motive s)
-: ∀ {s}, Abt₁ O s → motive s :=
-  @rec S O (λ s _ => motive s) (λ si _ => DList (motive ·.2) si) bvar var op DList.nil λ _ _ => DList.cons (α := _ × S) (β := (motive ·.2))
-
-end Abt₁
-
-variable {S : Type} (O : ∀ ⦃n⦄, (Fin n → List S × S) → S → Type) in
-inductive Abt₂ : S → Type
-  | bvar s (n : Nat) : Abt₂ s
-  | var (x : Var s) : Abt₂ s
-  | op (o : @O n si s) (ai : ∀ i, Abt₂ (si i).2) : Abt₂ s
-
-variable {S : Type} (O : ∀ ⦃n⦄, (Fin n → ((m : Nat) × (Fin m → S)) × S) → S → Type) in
-inductive Abt₃ : S → Type
-  | bvar s (n : Nat) : Abt₃ s
-  | var (x : Var s) : Abt₃ s
-  | op (o : @O n si s) (ai : ∀ i, Abt₃ (si i).2) : Abt₃ s
-
-def Abt₁.subst [DecidableEq S] {s : S} (a : Abt₁ O s) (x : Var s) : Abt₁ O t → Abt₁ O t :=
-  ndrec
-    (λ t n => bvar t n)
-    (λ {t} y => if h : t = s then if h ▸ y = x then h ▸ a else var y else var y)
-    (λ o _ ai' => op o ai')
-
-variable [DecidableEq S] {s : S} (a : Abt₂ O s) (x : Var s) in
-def Abt₂.subst : Abt₂ O t → Abt₂ O t
-  | bvar t n => bvar t n
-  | var y => if h : t = s then if h ▸ y = x then h ▸ a else var y else var y
-  | op o ai => op o λ i => subst (ai i)
-
-variable [DecidableEq S] {s : S} (a : Abt₃ O s) (x : Var s) in
-def Abt₃.subst : Abt₃ O t → Abt₃ O t
-  | bvar t n => bvar t n
-  | var y => if h : t = s then if h ▸ y = x then h ▸ a else var y else var y
-  | op o ai => op o λ i => subst (ai i)
-
-variable [DecidableEq S] (s : S) in
-def bindCount : List S → Nat
-  | [] => 0
-  | t :: ts => bindCount ts + if t = s then 1 else 0
-
-variable {S : Type u} [DecidableEq S] (s : S) in
-def bindCount' : ((m : Nat) × (Fin m → S)) → Nat
-  | ⟨0, _⟩ => 0
-  | ⟨m + 1, ts⟩ => bindCount' ⟨m, ts ∘ .succ⟩ + if ts .zero = s then 1 else 0
-
-def Abt₁.bind [DecidableEq S] {s : S} (x : Var s) : @Abt₁ S O t → Nat → Abt₁ O t :=
-  ndrec (motive := λ t => Nat → Abt₁ O t)
-    (λ t m _ => bvar t m)
-    (λ {t} y n => if h : t = s then if h ▸ y = x then bvar t n else var y else var y)
-    (λ o _ ai' n => op o (ai'.map λ {b} f => f (n + bindCount s b.1)))
-
-variable [DecidableEq S] {s : S} (x : Var s) in
-def Abt₂.bind (n : Nat) : @Abt₂ S O t → Abt₂ O t
-  | bvar t m => bvar t m
-  | var y => if h : t = s then if h ▸ y = x then bvar t n else var y else var y
-  | op (si := si) o ai => op o λ i => bind (n + bindCount s (si i).1) (ai i)
-
-variable [DecidableEq S] {s : S} (x : Var s) in
-def Abt₃.bind (n : Nat) : @Abt₃ S O t → Abt₃ O t
-  | bvar t m => bvar t m
-  | var y => if h : t = s then if h ▸ y = x then bvar t n else var y else var y
-  | op (si := si) o ai => op o λ i => bind (n + bindCount' s (si i).1) (ai i)
-
-def Abt₁.op' [DecidableEq S] {s : S} (o : O si s) (ai : DList (λ b => DList Var b.1 × Abt₁ O b.2) si) : Abt₁ O s :=
-  .op o <| ai.map λ a => a.1.foldr (λ {t} x (a, n) => (bind x a (n t), λ u => if u = t then n u + 1 else n u)) (a.2, λ _ : S => 0) |>.1
-
-def Abt₂.op' [DecidableEq S] {s : S} (o : O si s) (ai : ∀ i, DList Var (si i).1 × Abt₂ O (si i).2) : Abt₂ O s :=
-  .op o λ i => (ai i).1.foldr (λ {t} x (a, n) => (bind x (n t) a, λ u => if u = t then n u + 1 else n u)) ((ai i).2, λ _ : S => 0) |>.1
-
-def Abt₃.op' [DecidableEq S] {s : S} (o : O si s) (ai : ∀ i, (∀ j, Var ((si i).1.2 j)) × Abt₃ O (si i).2) : Abt₃ O s :=
-  .op o λ i => FinTuple.foldr (λ {j} x (a, n) => let t := (si i).1.2 j; (bind x (n t) a, λ u => if u = t then n u + 1 else n u)) ((ai i).2, λ _ : S => 0) (ai i).1 |>.1
-
-inductive O₁ : List (List Unit × Unit) → Unit → Type
-  | foo : O₁ [([], ()), ([], ())] ()
-  | bar : O₁ [([(), ()], ())] ()
-
-instance : ToString (O₁ si s) where
-  toString
-  | .foo => "foo"
-  | .bar => "bar"
-
-open FinTuple in
-inductive O₂ : ∀ ⦃n⦄, (Fin n → List Unit × Unit) → Unit → Type
-  | foo : O₂ ⟦([], ()), ([], ())⟧ ()
-  | bar : O₂ ⟦([(), ()], ())⟧ ()
-
-instance : ToString (O₂ si s) where
-  toString
-  | .foo => "foo"
-  | .bar => "bar"
-
-open FinTuple in
-inductive O₃ : ∀ ⦃n⦄, (Fin n → ((m : Nat) × (Fin m → Unit)) × Unit) → Unit → Type
-  | foo : O₃ ⟦(⟨_, ⟦⟧⟩, ()), (⟨_, ⟦⟧⟩, ())⟧ ()
-  | bar : O₃ ⟦(⟨_, ⟦(), ()⟧⟩, ())⟧ ()
-
-instance : ToString (O₃ si s) where
-  toString
-  | .foo => "foo"
-  | .bar => "bar"
-
-variable {S : Type} {O : ∀ ⦃n⦄, (Fin n → List S × S) → S → Type} in
-instance [DecidableEq S] [∀ {n} si s, ToString (@O n si s)] : ToString (Abt₂ O s) where
-  toString a := h (λ _ => 0) a
-where
-  h {s} (d : S → Nat) : Abt₂ O s → String
-  | .var x => x.toString ++ "'"
-  | .bvar s (x : Nat) => Var.toString (s := s) ⟨d s - 1 - x⟩
-  | .op (si := si) o ai => toString o ++ h' λ i => h'' d (si i).1 ++ h (λ s' => d s' + bindCount s' (si i).1) (ai i)
-  h' : ∀ {n}, (Fin n → String) → String
-  | 0, _ => ""
-  | _ + 1, ai => "(" ++ String.join (List.intersperse "; " (FinTuple.toList ai)) ++ ")"
-  h'' (d : S → Nat) : List S → String
-  | [] => ""
-  | si => String.join (List.intersperse ", " (si.foldl (λ (bs, d) b => (Var.toString (s := b) ⟨d b⟩ :: bs, λ s => d s + if b = s then 1 else 0)) ([], d)).1.reverse) ++ ". "
-
-variable {S : Type} {O : ∀ ⦃n⦄, (Fin n → ((m : Nat) × (Fin m → S)) × S) → S → Type} in
-instance [DecidableEq S] [∀ {n} si s, ToString (@O n si s)] : ToString (Abt₃ O s) where
-  toString a := h (λ _ => 0) a
-where
-  h {s} (d : S → Nat) : Abt₃ O s → String
-  | .var x => x.toString ++ "'"
-  | .bvar s (x : Nat) => Var.toString (s := s) ⟨d s - 1 - x⟩
-  | .op (si := si) o ai => toString o ++ h' λ i => h'' d (si i).1 ++ h (λ s' => d s' + bindCount' s' (si i).1) (ai i)
-  h' : ∀ {n}, (Fin n → String) → String
-  | 0, _ => ""
-  | _ + 1, ai => "(" ++ String.join (List.intersperse "; " (FinTuple.toList ai)) ++ ")"
-  h'' (d : S → Nat) : (m : Nat) × (Fin m → S) → String
-  | ⟨0, _⟩ => ""
-  | ⟨_ + 1, si⟩ => String.join (List.intersperse ", " (FinTuple.foldl (λ (bs, d) b => (Var.toString (s := b) ⟨d b⟩ :: bs, λ s => d s + if b = s then 1 else 0)) ([], d) si).1.reverse) ++ ". "
-
-open DList in
-#reduce (.op' .bar ⟦(⟦23, 24⟧, .op .foo ⟦.var 23, .var 24⟧)⟧ : Abt₁ O₁ ())
-open FinTuple DList in
-#eval (.op' .bar ⟦(⟦"x", "y"⟧, .op .foo ⟦.var "x", .var "y"⟧)⟧ : Abt₂ O₂ ())
-open FinTuple in
-#eval (.op' .bar ⟦(⟦"x", "y"⟧, .op .foo ⟦.var "x", .var "y"⟧)⟧ : Abt₃ O₃ ())
-
-/-
-def Abt.free [DecidableEq S] (s' : S) (a : Abt S O s) : Var' s' :=
-  let n := fv a
-  let v := h a (mkArray n true)
-  Id.run do
-  for (i, b) in v.toList.enum do
-    if b then
-      return ⟨i⟩
-  return ⟨n⟩
-where
-  fv {s}
-  | .fvar (s := s'') _ => if s'' = s' then 1 else 0
-  | .var _ _ => 0
-  | .op _ ai => FinTuple.foldr Nat.add 0 λ i => fv (ai i)
-  h {s}
-  | .fvar (s := s'') x, v => if s'' = s' then v.setD x.x false else v
-  | .var _ _, v => v
-  | .op _ ai, v => FinTuple.foldr (λ (f : _ → _) a => f a) v λ i => h (ai i)
-
-def Abt.unbind [DecidableEq S] {s' : S} (x : Var' s') (d : Nat) : Abt S O s → Abt S O s
-  | .fvar y => .fvar y
-  | .var s (y : Nat) =>
-    if h : s = s'
-    then
-      match compare y d with
-      | .gt => .var s (y - 1)
-      | .eq => h ▸ .fvar x
-      | .lt => .var s y
-    else .var s y
-  | .op (si := si) o ai => .op o λ i => (ai i).unbind x (d + liftAmt s' (si i).1)
-
-def Abt.unop [DecidableEq S] (o : O si s) (ai : ∀ i, Abt S O (si i).2) i : (∀ j, Var' ((si i).1.2 j)) × Abt S O (si i).2 :=
-  FinTuple.dfoldl
-    (β := λ k => (S → Nat) × ((j : Fin k) → Var' ((si i).1.2 (j.cast (Nat.pred_le_pred k.isLt)))) × Abt S O (si i).2)
-    (λ {j} (d, f, a) _ => let b := (si i).1.2 j; let x := a.free b; let d' s := if s = b then d s - 1 else d s; (d', Fin.revCases x f, a.unbind x (d' b)))
-    ((liftAmt · (si i).1), λ k => nomatch k, ai i)
-    (si i).1.2
-    |>.2
-
-instance (priority := low) [ToString α] : Repr α where
-  reprPrec x _ := toString x
 
 namespace ExampleAbt
 
@@ -534,112 +842,415 @@ inductive S
   | Exp
 deriving DecidableEq
 
-inductive O : ∀ ⦃n⦄, (Fin n → ((m : Nat) × (Fin m → S)) × S) → S → Type
-  | num : Nat → O ⟦⟧ .Exp
-  | plus : O ⟦(⟦⟧', .Exp), (⟦⟧', .Exp)⟧ .Exp
-  | times : O ⟦(⟦⟧', .Exp), (⟦⟧', .Exp)⟧ .Exp
-  | let : O ⟦(⟦⟧', .Exp), (⟦.Exp⟧', .Exp)⟧ .Exp
-
-abbrev Abt := _root_.Abt S O
+inductive O : List (List S × S) → S → Type
+  | num : Nat → O [] .Exp
+  | plus : O [([], .Exp), ([], .Exp)] .Exp
+  | times : O [([], .Exp), ([], .Exp)] .Exp
+  | let : O [([], .Exp), ([.Exp], .Exp)] .Exp
 
 instance : ToString (O si s) where
-  toString := h
-where h
+  toString
   | .num n => s!"num[{n}]"
   | .plus => "plus"
   | .times => "times"
   | .let => "let"
 
-inductive Exp
-  | var : Var' S.Exp → Exp
-  | num : Nat → Exp
-  | plus : Abt .Exp → Abt .Exp → Exp
-  | times : Abt .Exp → Abt .Exp → Exp
-  | let : Abt .Exp → Var' S.Exp → Abt .Exp → Exp
-  deriving Repr
+def Abt := WfAbt O
 
-def Exp.in : Exp → Abt .Exp
-  | .var x => .fvar x
+def Exp := Abt .Exp
+
+inductive Exp.View
+  | var : Var S.Exp → View
+  | num : Nat → View
+  | plus : Exp → Exp → View
+  | times : Exp → Exp → View
+  | let : Exp → Var S.Exp → Exp → View
+
+open DList
+
+def Exp.in : View → Exp
+  | .var x => .var ⟨_, _, .let, [.Exp], by simp⟩ x
   | .num n => .op (.num n) ⟦⟧ 
   | .plus a b => .op .plus ⟦a, b⟧
   | .times a b => .op .times ⟦a, b⟧
   | .let a x b => .op' .let ⟦(⟦⟧, a), (⟦x⟧, b)⟧
 
-def Exp.out : Abt .Exp → Exp
-  | .fvar x => .var x
-  | .var _ x => .var ⟨x⟩
-  | .op (.num n) _ => .num n 
-  | .op .plus ai => .plus (ai 0) (ai 1)
-  | .op .times ai => .times (ai 0) (ai 1)
-  | .op .let ai => let ai' := Abt.unop .let ai; .let (ai' 0).2 ((ai' 1).1 .zero) (ai' 1).2
+def Exp.out (e : Exp) : View :=
+  match WfAbt.out e with
+  | .var _ x => .var x
+  | .op (.num n) ⟦⟧ => .num n 
+  | .op .plus ⟦(⟦⟧, a), (⟦⟧, b)⟧ => .plus a b
+  | .op .times ⟦(⟦⟧, a), (⟦⟧, b)⟧ => .times a b
+  | .op .let ⟦(⟦⟧, a), (⟦x⟧, b)⟧ => .let a x b
 
-def Exp'.var := (Exp.in <| Exp.var ·)
-def Exp'.num := (Exp.in <| Exp.num ·)
-def Exp'.plus := (Exp.in <| Exp.plus · ·)
-def Exp'.times := (Exp.in <| Exp.times · ·)
-def Exp'.let := (Exp.in <| Exp.let · · ·)
+def Exp.var := («in» <| .var ·)
+def Exp.num := («in» <| .num ·)
+def Exp.plus := («in» <| .plus · ·)
+def Exp.times := («in» <| .times · ·)
+def Exp.let := («in» <| .let · · ·)
 
-theorem Exp.in_out : ∀ e, Exp.in (Exp.out e) = e
-  | .fvar x => rfl
-  | .var _ x => sorry
-  | .op (.num n) _ => congrArg (Abt.op _) <| funext λ i => nomatch i
-  | .op .plus ai => congrArg (Abt.op _) <| funext λ | 0 => rfl | 1 => rfl
-  | .op .times ai => congrArg (Abt.op _) <| funext λ | 0 => rfl | 1 => rfl
-  | .op .let ai => congrArg (Abt.op _) <| funext λ | 0 => rfl | 1 => sorry
+theorem Exp.in_out : ∀ e, «in» (out e) = e
+  | ⟨.var .., _⟩ => rfl
+  | ⟨.op (.num _) ⟦⟧, _⟩ => rfl
+  | ⟨.op .plus ⟦_, _⟧, _⟩ => rfl
+  | ⟨.op .times ⟦_, _⟧, _⟩ => rfl
+  | ⟨.op .let ⟦_, _⟧, wf⟩ => (WfAbt.in_out ⟨.op .let ⟦_, _⟧, wf⟩ :)
+
+variable {α} (num : Nat → α) (plus : α → α → α) (times : α → α → α) («let» : α → ((x : Exp) → x.1.closed (λ _ => False) → α) → α) in
+partial def Exp.evalClosed [Nonempty α] : (e : Exp) → e.1.closed (λ _ => False) → α
+  | ⟨.var .., _⟩ => False.elim
+  | ⟨.op (.num n) ⟦⟧, _⟩ => λ _ => num n
+  | ⟨.op .plus ⟦a, b⟧, wfa, wfb, _⟩ => λ ⟨ca, cb, _⟩ => plus (evalClosed ⟨a, wfa⟩ ca) (evalClosed ⟨b, wfb⟩ cb)
+  | ⟨.op .times ⟦a, b⟧, wfa, wfb, _⟩ => λ ⟨ca, cb, _⟩ => times (evalClosed ⟨a, wfa⟩ ca) (evalClosed ⟨b, wfb⟩ cb)
+  | ⟨.op .let ⟦a, b⟧, wfa, (wfb : Abt.wellFormed _ _), _⟩ => λ ⟨ca, cb, _⟩ => «let» (evalClosed ⟨a, wfa⟩ ca) λ x cx => evalClosed ⟨Abt.unbind x.1 b 0, Abt.wellFormed_unbind x.2 .refl <| by simp [Abt.bindCount] at wfb ⊢; exact wfb⟩ (Abt.closed_unbind (λ _ => False) cx cb)
+
+def Exp.eval : (e : Exp) → (_ : e.1.closed (λ _ => False) := by decide) → Nat :=
+  evalClosed
+    (λ n => n)
+    (λ a b => a + b)
+    (λ a b => a * b)
+    (λ a b => b (num a) ⟨⟩)
+
+open Exp in
+#eval «let» (plus (num 2) (num 3)) "z" (times (var "z") (num 8))
+open Exp in
+#eval eval (.let (plus (num 2) (num 3)) "z" (times (var "z") (num 8)))
 
 end ExampleAbt
 
-section
-open ExampleAbt Exp'
-#eval Exp'.let (plus (num 2) (num 3)) "z" (times (var "z") (num 5))
-#eval match Exp'.let (plus (num 2) (num 3)) "z" (times (var "z") (num 5)) with | .op .let ai => Abt.unop O.let ai | _ => unreachable!
-end
+namespace ULC
 
-inductive O : ∀ ⦃n⦄, (Fin n → ((m : Nat) × (Fin m → Unit)) × Unit) → Unit → Type
-  | zero : O ⟦(⟦⟧', ()), (⟦⟧', ())⟧ ()
-  | one : O ⟦(⟦()⟧', ())⟧ ()
-  | two : O ⟦(⟦(), ()⟧', ())⟧ ()
+inductive S
+  | Exp
+deriving DecidableEq
+
+inductive O : List (List S × S) → S → Type
+  | abs : O [([.Exp], .Exp)] .Exp
+  | app : O [([], .Exp), ([], .Exp)] .Exp
 
 instance : ToString (O si s) where
   toString
-    | .zero => "zero"
-    | .one => "one"
-    | .two => "two"
+    | .abs => "abs"
+    | .app => "app"
 
-#eval Abt.op' O.one ⟦(⟦"x"⟧, .fvar "x")⟧
-#eval Abt.op' O.one ⟦(⟦"x"⟧, .fvar "y")⟧
-#eval Abt.op' O.two ⟦(⟦"x", "y"⟧, .fvar "x")⟧
-#eval Abt.op' O.two ⟦(⟦"x", "y"⟧, .fvar "y")⟧
-#eval Abt.op' O.two ⟦(⟦"x", "y"⟧, .fvar "z")⟧
-#eval Abt.op' O.two ⟦(⟦"x", "y"⟧, .op' .zero ⟦(⟦⟧, .fvar "x"), (⟦⟧, .fvar "y")⟧)⟧
+abbrev Abt := WfAbt O
 
-#eval match Abt.op' O.two ⟦(⟦"x", "y"⟧, .fvar "x")⟧ with | .op .two ai => Abt.unop O.two ai | _ => unreachable!
-#eval match Abt.op' O.two ⟦(⟦"x", "y"⟧, .fvar "y")⟧ with | .op .two ai => Abt.unop O.two ai | _ => unreachable!
-#eval match Abt.op' O.two ⟦(⟦"x", "y"⟧, .fvar "z")⟧ with | .op .two ai => Abt.unop O.two ai | _ => unreachable!
-#eval match Abt.op' O.two ⟦(⟦"x", "y"⟧, .op' .zero ⟦(⟦⟧, .fvar "y"), (⟦⟧, .fvar "x")⟧)⟧ with | .op .two ai => Abt.unop O.two ai | _ => unreachable!
+abbrev Exp := Abt .Exp
 
-#eval Abt.op' O.one ⟦(⟦"x"⟧, .op' .one ⟦(⟦"y"⟧, .op .zero ⟦.fvar "x", .fvar "y"⟧)⟧)⟧
-#eval match Abt.op' O.one ⟦(⟦"x"⟧, .op' .one ⟦(⟦"y"⟧, .op .zero ⟦.fvar "x", .fvar "y"⟧)⟧)⟧ with | .op .one ai => Abt.unop O.one ai | _ => unreachable!
-#eval match Abt.op' O.one ⟦(⟦"x"⟧, .op' .one ⟦(⟦"y"⟧, .op .zero ⟦.fvar "x", .fvar "y"⟧)⟧)⟧ with | .op .one ai => (match Abt.unop O.one ai 0 |>.2 with | .op .one ai => Abt.unop O.one ai | _ => unreachable!) | _ => unreachable!
+inductive Exp.View
+  | var : Var S.Exp → View
+  | abs : Var S.Exp → Exp → View
+  | app : Exp → Exp → View
 
-/-
-variable (S : Type) (O : ∀ ⦃n⦄, (Fin n → (S → Nat) × S) → S → Type) in
-inductive CAbt : (S → Nat) → S → Type
-  | var s (x : Fin (X s)) : CAbt X s
-  | op (o : O si s) (ai : ∀ i, CAbt (λ s => X s + (si i).1 s) (si i).2) : CAbt X s
+open DList
 
-def ClAbt S O := CAbt S O λ _ => 0
--/
+def Exp.in : View → Exp
+  | .var x => .var ⟨_, _, .abs, [.Exp], by simp⟩ x
+  | .abs x e => .op' .abs ⟦(⟦x⟧, e)⟧
+  | .app e₁ e₂ => .op .app ⟦e₁, e₂⟧
 
-/-
-def Nat.le.rec' {n} {motive : (a : Nat) → n.le a → Sort u}
-  (refl : motive n .refl)
-  (step : ∀ {m} a, motive m a → motive m.succ a.step) {a} t
-: motive a t := by
-  cases h : a - n
-    <;> have := Nat.sub_add_cancel t |>.symm |>.trans <| congrArg (· + n) h
-    <;> simp [this, Nat.succ_add]
-  . exact refl
-  . exact step (Nat.le_add_left n _) (rec' refl step _)
-  -/
--/
+def Exp.var := (Exp.in <| .var ·)
+def Exp.abs := (Exp.in <| .abs · ·)
+def Exp.app := (Exp.in <| .app · ·)
+
+def Exp.out (e : Exp) : View :=
+  match WfAbt.out e with
+  | .var _ x => .var x
+  | .op .abs ⟦(⟦x⟧, e)⟧ => .abs x e
+  | .op .app ⟦(⟦⟧, e₁), (⟦⟧, e₂)⟧ => .app e₁ e₂
+
+end ULC
+
+open ULC in
+#eval Exp.app (.abs "x" <| .var "x") (.abs "x" <| .var "x")
+
+namespace E
+
+inductive S
+  | Typ
+  | Exp
+deriving DecidableEq
+
+inductive O : List (List S × S) → S → Type
+  | arr : O [([], .Typ), ([], .Typ)] .Typ
+  | void : O [] .Typ
+  | lam : O [([], .Typ), ([.Exp], .Exp)] .Exp
+  | ap : O [([], .Exp), ([], .Exp)] .Exp
+deriving DecidableEq
+
+instance : ToString (O si s) where
+  toString
+    | .arr => "arr"
+    | .void => "void"
+    | .lam => "lam"
+    | .ap => "ap"
+
+abbrev Abt := WfAbt O
+
+abbrev Typ := Abt .Typ
+abbrev Exp := Abt .Exp
+
+inductive Typ.View
+  | arr : Typ → Typ → View
+  | void : View
+
+inductive Exp.View
+  | var : Var S.Exp → View
+  | lam : Var S.Exp → Typ → Exp → View
+  | ap : Exp → Exp → View
+
+open DList
+
+def Typ.in : View → Typ
+  | .arr τ₁ τ₂ => .op .arr ⟦τ₁, τ₂⟧
+  | .void => .op .void ⟦⟧
+
+def Typ.arr := (Typ.in <| .arr · ·)
+def Typ.void := (Typ.in <| .void)
+
+theorem Typ.notBound : ¬isBound O S.Typ := by
+    intro h
+    match h with
+    | ⟨_, _, .arr, b, .tail _ <| .tail _ h, _⟩ => cases h
+    | ⟨_, _, .lam, b, .tail _ <| .tail _ h, _⟩ => cases h
+    | ⟨_, _, .ap, b, .tail _ <| .tail _ h, _⟩ => cases h
+
+def Typ.out (τ : Typ) : View :=
+  match WfAbt.out τ with
+  | .var h _ => notBound h |>.elim
+  | .op .arr ⟦(⟦⟧, τ₁), (⟦⟧, τ₂)⟧ => .arr τ₁ τ₂
+  | .op .void ⟦⟧ => .void
+
+theorem Typ.in_out : ∀ τ, «in» (out τ) = τ
+  | ⟨.var h _, _⟩ => notBound h |>.elim
+  | ⟨.op .arr ⟦_, _⟧, _⟩ => rfl
+  | ⟨.op .void ⟦⟧, _⟩ => rfl
+
+theorem Typ.out_in : ∀ τ, out («in» τ) = τ
+  | .arr .. => rfl
+  | .void => rfl
+
+def Exp.in : View → Exp
+  | .var x => .var ⟨_, _, .lam, [.Exp], by simp⟩ x
+  | .lam x τ e => .op' .lam ⟦(⟦⟧, τ), (⟦x⟧, e)⟧
+  | .ap e₁ e₂ => .op .ap ⟦e₁, e₂⟧
+
+def Exp.var := (Exp.in <| .var ·)
+def Exp.lam := (Exp.in <| .lam · · ·)
+def Exp.ap := (Exp.in <| .ap · ·)
+
+def Exp.out (e : Exp) : View :=
+  match WfAbt.out e with
+  | .var _ x => .var x
+  | .op .lam ⟦(⟦⟧, τ), (⟦x⟧, e)⟧ => .lam x τ e
+  | .op .ap ⟦(⟦⟧, e₁), (⟦⟧, e₂)⟧ => .ap e₁ e₂
+
+theorem Exp.in_out : ∀ e, «in» (out e) = e
+  | ⟨.var .., _⟩ => rfl
+  | ⟨.op .lam ⟦_, _⟧, wf⟩ => (WfAbt.in_out ⟨.op .lam ⟦_, _⟧, wf⟩ :)
+  | ⟨.op .ap ⟦_, _⟧, _⟩ => rfl
+
+protected partial def Typ.toString (τ : Typ) : String :=
+  match Typ.out τ with
+  | .arr τ₁ τ₂ => s!"({τ₁.toString} → {τ₂.toString})"
+  | .void => "void"
+
+protected partial def Exp.toString (e : Exp) : String :=
+  match Exp.out e with
+  | .var x => toString x
+  | .lam x τ e => s!"(λ {x} : {τ.toString}. {e.toString})"
+  | .ap e₁ e₂ => s!"({e₁.toString} {e₂.toString})"
+
+instance : ToString Typ := ⟨Typ.toString⟩
+
+instance : ToString Exp := ⟨Exp.toString⟩
+
+variable {motive : Exp → Sort u} (var : ∀ x, motive (var x)) (lam : ∀ x τ e, motive e → motive (lam x τ e)) (ap : ∀ e₁ e₂, motive e₁ → motive e₂ → motive (ap e₁ e₂)) in
+@[eliminator, elab_as_elim]
+def Exp.rec (e : Exp) : motive e :=
+  match h : WfAbt.out e with
+  | .var v x => by apply Eq.mp _ <| var x; show motive (WfAbt.View.in (.var v x)) = motive e; rw [← h, WfAbt.in_out]
+  | .op .lam ⟦(⟦⟧, τ), (⟦x⟧, e')⟧ =>
+    have h' : τ.1.sizeOf + e'.1.sizeOf + 1 = e.1.sizeOf := (h ▸ WfAbt.sizeOf_out _ :)
+    have : e'.1.sizeOf < e.1.sizeOf := Nat.lt_of_lt_add_left <| Nat.le_of_eq h'
+    by apply Eq.mp _ <| lam x τ e' (rec e'); show motive (WfAbt.View.in (.op .lam ⟦(⟦⟧, τ), (⟦x⟧, e')⟧)) = motive e; rw [← h, WfAbt.in_out]
+  | .op .ap ⟦(⟦⟧, e₁), (⟦⟧, e₂)⟧ =>
+    have h' : e₁.1.sizeOf + e₂.1.sizeOf + 1 = _ := h ▸ WfAbt.sizeOf_out _
+    have : e₁.1.sizeOf < e.1.sizeOf := Nat.lt_of_lt_add_right (by exact Nat.le_of_eq h')
+    have : e₂.1.sizeOf < e.1.sizeOf := Nat.lt_of_lt_add_left (by exact Nat.le_of_eq h')
+    by apply Eq.mp _ <| ap e₁ e₂ (rec e₁) (rec e₂); show motive (WfAbt.View.in (.op .ap ⟦(⟦⟧, e₁), (⟦⟧, e₂)⟧)) = motive e; rw [← h, WfAbt.in_out]
+termination_by _ e => e.1.sizeOf
+
+variable {motive : Exp.View → Sort u} (var : ∀ x, motive (.var x)) (lam : ∀ x τ e, motive e.out → motive (.lam x τ e)) (ap : ∀ e₁ e₂, motive e₁.out → motive e₂.out → motive (.ap e₁ e₂)) in
+def Exp.rec' (e : Exp) : motive e.out :=
+  match h : e.out with
+  | .var x => var x
+  | .lam x τ e' =>
+    have h' : τ.1.sizeOf + e'.1.sizeOf + 1 = e.1.sizeOf := have h : WfAbt.out e = .op .lam ⟦(⟦⟧, τ), (⟦x⟧, e')⟧ := by { unfold out at h; split at h <;> cases h; assumption }; (h ▸ WfAbt.sizeOf_out _ :)
+    have : e'.1.sizeOf < e.1.sizeOf := Nat.lt_of_lt_add_left <| Nat.le_of_eq h'
+    lam x τ e' (rec' e')
+  | .ap e₁ e₂ =>
+    have h' : e₁.1.sizeOf + e₂.1.sizeOf + 1 = _ := have h : WfAbt.out e = .op .ap ⟦(⟦⟧, e₁), (⟦⟧, e₂)⟧ := by { unfold out at h; split at h <;> cases h; assumption }; h ▸ WfAbt.sizeOf_out _
+    have : e₁.1.sizeOf < e.1.sizeOf := Nat.lt_of_lt_add_right (by exact Nat.le_of_eq h')
+    have : e₂.1.sizeOf < e.1.sizeOf := Nat.lt_of_lt_add_left (by exact Nat.le_of_eq h')
+    ap e₁ e₂ (rec' e₁) (rec' e₂)
+termination_by _ e => e.1.sizeOf
+
+inductive Typing : List (Var S.Exp × Typ) → Exp.View → Typ → Prop
+  | var : Γ.lookup x = some τ → Typing Γ (.var x) τ
+  | lam : Typing ((x, τ) :: Γ) e.out τ' → Typing Γ (.lam x τ e) (.arr τ τ')
+  | ap : Typing Γ e₁.out (.arr τ₁ τ₂) → Typing Γ e₂.out τ₁ → Typing Γ (.ap e₁ e₂) τ₂
+
+theorem Typing.uniqueness : ∀ {τ}, Typing Γ e τ → ∀ {τ'}, Typing Γ e τ' → τ = τ' := Typing.rec (motive := λ Γ e τ _ => ∀ τ', Typing Γ e τ' → τ = τ')
+  (λ h _ (.var h') => Option.some.inj <| h.symm.trans h')
+  (λ _ ih _ (.lam h') => ih _ h' ▸ rfl)
+  (λ _ _ ih₁ _ _ (.ap h₁' _) => And.right <| Typ.View.arr.inj <| congrArg Typ.out (ih₁ _ h₁'))
+
+def inferType : ∀ (e : Exp) Γ, Option { τ // Typing Γ e.out τ } := Exp.rec
+  (λ x Γ =>
+    match h : Γ.lookup x with
+    | some τ => some ⟨τ, .var h⟩
+    | none => none
+  )
+  (λ x τ _ inferType_e Γ =>
+    match inferType_e ((x, τ) :: Γ) with
+    | some ⟨τ', h⟩ => some ⟨.arr τ τ', .lam h⟩
+    | none => none
+  )
+  (λ _ _ inferType_e₁ inferType_e₂ Γ =>
+    match inferType_e₁ Γ, inferType_e₂ Γ with
+    | some ⟨τ₁, h₁⟩, some ⟨τ₂, h₂⟩ =>
+      match h₁' : τ₁.out with
+      | .arr τ τ' =>
+        if h : τ = τ₂
+        then some ⟨τ', .ap ((congrArg _ (h ▸ Typ.in_out _ ▸ congrArg Typ.in h₁' :)).mp h₁) h₂⟩
+        else none
+      | _ => none
+    | _, _ => none
+  )
+
+inductive InferTypeResult₁ Γ e
+  | success τ (h : Typing₁ Γ e τ)
+  | failure (h : ∀ τ, ¬Typing₁ Γ e τ)
+
+inductive InferTypeResult₂ Γ e
+  | success τ (h : Typing₂ Γ e τ)
+  | failure (h : ∀ τ, ¬Typing₂ Γ e τ)
+
+def inferType₁ : ∀ e Γ, InferTypeResult₁ Γ (Exp.out e) := @Exp.rec' (λ e => ∀ Γ, InferTypeResult₁ Γ e)
+  (λ x Γ =>
+    match h : Γ.lookup x with
+    | some τ => .success τ (.var h)
+    | none => .failure λ _ (.var h') => nomatch (h.symm.trans h')
+  )
+  (λ x τ e inferType_e Γ =>
+    match inferType_e ((x, τ) :: Γ) with
+    | .success τ' h => .success (.arr τ τ') (.lam h)
+    | .failure h => .failure λ _ (.lam h') => h _ h'
+  )
+  (λ e₁ e₂ inferType_e₁ inferType_e₂ Γ =>
+    match inferType_e₁ Γ, inferType_e₂ Γ with
+    | .success τ₁ h₁, .success τ₂ h₂ =>
+      match h₁' : τ₁.out with
+      | .arr τ τ' => sorry
+      | _ => .failure λ _ (.ap h₁' _) => sorry
+    | .failure h₁, _ => .failure λ _ (.ap h₁' _) => h₁ _ h₁'
+    | _, .failure h₂ => .failure λ _ (.ap _ h₂') => h₂ _ h₂'
+  )
+
+end E
+
+open E in
+#eval Exp.ap (.lam "f" (.arr .void .void) <| .lam "x" .void <| .ap (.var "f") <| .ap (.var "f") <| .var "x") (.lam "x" .void <| .var "x")
+
+open E in
+#eval Exp.ap (.lam "f" .void <| .ap (.var "f") (.var "f")) (.lam "x" .void <| .var "x")
+
+open E in
+#eval inferType (.lam "x" .void <| .ap (.var "f") (.var "x")) [("f", .arr .void .void)]
+
+open E in
+#eval Typ.arr (.arr .void .void) (.arr .void .void)
+
+namespace Ast
+
+scoped syntax "ast " ident manyIndent(ident manyIndent("| " ident (colGt ident <|> str <|> Lean.Parser.Term.paren)*)) : command
+
+macro_rules
+  | `(ast $name $[$sort $[| $ctor $args*]*]*) => do
+    let args : Array (Array (Array (Lean.TSyntax `term × _))) ← args.mapM <| Array.mapM <| Array.mapM λ arg =>
+      match arg.raw with
+      | `($arg:str) => return (arg, none)
+      | `($arg) => return (arg, some <| ← Lean.withFreshMacroScope `(x))
+    let argTypes := args.map <| Array.map <| Array.filterMap λ (t, x?) => x?.map λ _ => t
+    let ctorType ← (sort.zip argTypes).mapM λ (s, a) => a.mapM <| Array.foldrM (`($(·) → $(·))) (s : Lean.Ident)
+    let toString := sort.map (Lean.mkIdent <| ·.getId.str "toString")
+    let argVars := args.map <| Array.map <| Array.filterMap (·.2)
+    let fullCtor := (sort.zip ctor).map λ (s, c) => c.map (Lean.mkIdent <| s.getId ++ Lean.TSyntax.getId ·)
+    let ctorToString ← (ctor.zip args).mapM λ (c, a) => (c.zip a).mapM λ (c, a) =>
+      a.foldlM (λ s (t, x?) =>
+        match x? with
+        | some x =>
+          if sort.contains ⟨t.raw⟩
+          then `($s ++ $(x).toString)
+          else `($s ++ toString $x)
+        | none => `($s ++ $t)
+      ) (Lean.Syntax.mkStrLit c.getId.toString)
+    `(namespace $name
+      mutual
+      $[inductive $sort
+          $[| $ctor:ident : $ctorType]*]*
+      end
+      mutual
+      $[protected def $toString : $sort → String
+          $[| $fullCtor:ident $argVars* => $ctorToString]*]*
+      end
+      mutual
+      $[instance : ToString $sort := ⟨$toString⟩]*
+      end
+      end $name)
+
+end Ast
+
+open Ast in
+ast Example
+  Num
+  | num "[" Nat "]"
+  | plus "(" Num "; " Num ")"
+  | times "(" Num "; " Num ")"
+  | parse "(" Str ")"
+  Str
+  | str "[" String "]"
+  | concat "(" Str "; " Str ")"
+  | «repeat» "(" Str "; " Num ")"
+  | toStr "(" Num ")"
+
+def String.repeat : Nat → String → String
+  | 0, _ => ""
+  | 1, s => s
+  | n + 1, s => String.repeat n s ++ s
+
+namespace Example
+
+mutual
+
+def evalNum : Num → Nat
+  | .num n => n
+  | .plus n m => evalNum n + evalNum m
+  | .times n m => evalNum n * evalNum m
+  | .parse s => String.toNat! (evalStr s)
+
+def evalStr : Str → String
+  | .str s => s
+  | .concat s t => evalStr s ++ evalStr t
+  | .repeat s n => .repeat (evalNum n) (evalStr s)
+  | .toStr n => toString (evalNum n)
+
+end
+
+open Num Str
+
+#eval parse («repeat» (concat (str "1") (toStr (times (num 2) (num 3)))) (plus (num 2) (num 3)))
+#eval evalNum <| parse («repeat» (concat (str "1") (toStr (times (num 2) (num 3)))) (plus (num 2) (num 3)))
+
+end Example
