cps.lean
@@ -8,71 +8,95 @@ partial def getApp : Term → Term × Array Term
   | `(($t)) => getApp t
   | stx => (stx, #[])
 
-partial def cps' (i : Ident) (n : Nat) (a : Array Term → MacroM Term) (stx : Term) : MacroM ((Term → MacroM Term) × Term) :=
+variable (ns : NameMap (Nat × (Array Term → MacroM Term))) in
+partial def cps' (stx : Term) : MacroM ((Term → MacroM Term) × Term) :=
   let (hd, tl) := getApp stx
-  if hd == i then
+  --if let some (n, a) := ns.find? hd.raw.getId then
+  if !tl.isEmpty && ns.contains hd.raw.getId then
+    let (n, a) := ns.find! hd.raw.getId
     if tl.size < n
     then throw <| .error stx "function not fully applied"
     else do
       let (bs₁, tl₁) ← tl[:n].foldlM (λ (binds, tl) x => do
-        let (bind, y) ← cps' i n a x
+        let (bind, y) ← cps' x
         return (binds <=< bind, tl.push y)
       ) (pure, .mkEmpty n)
       let tl₁ ← a tl₁
       let (bs₂, tl₂) ← tl[n:].foldlM (λ (binds, tl) x => do
-        let (bind, y) ← cps' i n a x
+        let (bind, y) ← cps' x
         return (binds <=< bind, tl.push y)
       ) (pure, .mkEmpty (tl.size - n))
       let b ← withFreshMacroScope `(__do_lift)
       return (bs₁ <=< (λ bd => `($tl₁ >>= λ $b => $bd)) <=< bs₂, ← `($b $tl₂*))
   else if let `(← $e) := stx then do
-    let (be, e) ← cps' i n a e
+    let (be, e) ← cps' e
     let b ← withFreshMacroScope `(__do_lift)
     return (be <=< (λ bd => `($e >>= λ $b => $bd)), b)
   else if let `(if $c then $t else $e) := stx then do
-    let (bc, c) ← cps' i n a c
-    let (bt, t) ← cps' i n a t
-    let (be, e) ← cps' i n a e
+    let (bc, c) ← cps' c
+    let (bt, t) ← cps' t
+    let (be, e) ← cps' e
     let t ← bt <| ← `(pure $t)
     let e ← be <| ← `(pure $e)
     let b ← withFreshMacroScope `(__do_lift)
     return (bc <=< λ bd => `((if $c then $t else $e) >>= λ $b => $bd), b)
   else if let `(match $[$d],* with $[| $[$lhs,*]|* => $rhs]*) := stx then do
     let (bd, d) ← d.foldlM (λ (bd, d) arg => do
-      let (bind, arg') ← cps' i n a ⟨arg.raw[1]⟩
+      let (bind, arg') ← cps' ⟨arg.raw[1]⟩
       return (bd <=< bind, d.push ⟨arg.raw.setArg 1 arg'⟩)
     ) (pure, .mkEmpty d.size)
     let rhs ← rhs.mapM λ rhs => do
-      let (brhs, rhs) ← cps' i n a rhs
+      let (brhs, rhs) ← cps' rhs
       brhs <| ← `(pure $rhs)
     let b ← withFreshMacroScope `(__do_lift)
     return (bd <=< λ bd => `((match $[$d],* with $[| $[$lhs,*]|* => $rhs]*) >>= λ $b => $bd), b)
   else do
     let (binds, args) ← stx.raw.getArgs.foldlM (λ (binds, args) arg => do
-      let (bind, arg) ← cps' i n a ⟨arg⟩
+      let (bind, arg) ← cps' ⟨arg⟩
       return (binds <=< bind, args.push arg.raw)
     ) (pure, .mkEmpty stx.raw.getNumArgs)
     return (binds, ⟨stx.raw.setArgs args⟩)
 
 def cps (i : Ident) (n : Nat) (a : Array Term → MacroM Term := λ a => `($i $a*)) (t : Term) : MacroM Term := do
-  let (b, t) ← cps' i n a t
+  let (b, t) ← cps' (.insert .empty i.getId (n, a)) t
+  b <| ← `(pure $t)
+
+def cpsN (is : List (Ident × Nat)) (t : Term) : MacroM Term := do
+  let (b, t) ← cps' (.ofList <| is.map λ (i, n) => (i.getId, n, λ a => `($i $a*))) t
   b <| ← `(pure $t)
 
 /-
 macro "cps% " i:ident n:num t:term : term => (cps i n.getNat) t
 -/
 
-/-
 elab "#cps " i:ident n:num t:term : command => do
   let t' ← Elab.liftMacroM <| (cps i n.getNat) t
   logInfoAt t t'
--/
 
-/-
+syntax "#cps [" (ident num),* "]" term : command
+elab_rules : command | `(#cps [$[$i $n],*] $t) => do
+  let t' ← Elab.liftMacroM <| (cpsN (i.zip <| n.map TSyntax.getNat).toList) t
+  logInfoAt t t'
+
 elab tk:"#expand " t:term : command => do
   let t ← Elab.liftMacroM <| expandMacros t
   logInfoAt tk t
--/
+
+inductive Tree (α : Type u)
+  | leaf
+  | node (l : Tree α) (x : α) (r : Tree α)
+def Tree.map {α : Type u} {β : Type v} (f : α → β) : Tree α → Tree β
+  | leaf => leaf
+  | node l x r => node (map f l) (f x) (map f r)
+def Tree.mapA {m : Type v → Type w} [Applicative m] {α : Type u} {β : Type v} (f : α → m β) : Tree α → m (Tree β)
+  | leaf => pure leaf
+  | node l x r => node <$> mapA f l <*> f x <*> mapA f r
+def Tree.mapM {m : Type v → Type w} [Monad m] {α : Type u} {β : Type v} (f : α → m β) : Tree α → m (Tree β)
+  | leaf => return leaf
+  | node l x r => return node (← mapM f l) (← f x) (← mapM f r)
+
+#cps [map 2] leaf
+#cps [map 2, f 1] node (map f l) (f x) (map f r)
 
 def Function.curry (f : α × β → δ) (x : α) (y : β) : δ := f (x, y)
 
@@ -177,7 +201,7 @@ def mdef := leading_parser
 macro_rules
   | `(mdef $n : $t₁ → $t₂ $[| $[$l,*]|* => $r]*) => do
     let rs ← r.mapM <| cps n 1
-    `(def $n : $t₁ → $t₂ := λ
+    `(def $n : $t₁ → $t₂
       $[| $[$l,*]|* => $rs]*)
 
 def mul (x y : Nat) : Nat :=
