BTree.lean
@@ -1,0 +1,353 @@
+import Std.Data.List.Lemmas
+
+namespace List
+
+theorem Mem.of_mem_head : x ∈ head? l → x ∈ l := by
+  intro; cases l <;> simp_all
+
+theorem Mem.of_mem_last : x ∈ last' l → x ∈ l := by
+  match l with
+  | [] => simp
+  | [_] => intro; simp_all
+  | _ :: _ :: l => intro h; have := of_mem_last (l := _ :: l) h; simp_all
+
+@[simp]
+theorem last'_append_cons : (l ++ x :: r).last' = (x :: r).last' :=
+  match l with
+  | [] => rfl
+  | [_] => rfl
+  | _ :: _ :: l => last'_append_cons (l := _ :: l)
+
+@[simp]
+theorem head?_append_cons : (l ++ x :: r).head? = (l ++ [x]).head? := by
+  cases l <;> rfl
+
+variable {α : Type u} {R : α → α → Prop}
+
+@[simp] theorem Chain_nil_def : Chain R a [] ↔ True := ⟨λ | .nil => ⟨⟩, λ | ⟨⟩ => .nil⟩
+@[simp] theorem Chain_cons_def : Chain R a (b :: l) ↔ R a b ∧ Chain R b l := ⟨λ | .cons h h' => ⟨h, h'⟩, λ ⟨h, h'⟩ => .cons h h'⟩
+
+attribute [local simp] Chain'
+
+theorem Chain'_cons : Chain' R (x :: l) ↔ (∀ y ∈ l.head?, R x y) ∧ Chain' R l := by
+  cases l <;> simp
+
+theorem Chain'.cons (hx : ∀ y ∈ l.head?, R x y) (hl : Chain' R l) : Chain' R (x :: l) :=
+  Chain'_cons.mpr ⟨hx, hl⟩
+
+theorem Chain'_append : Chain' R (l ++ r) ↔ Chain' R l ∧ (∀ x ∈ l.last', ∀ y ∈ r.head?, R x y) ∧ Chain' R r := by
+  match l with
+  | [] => simp
+  | [x] => simp; exact Chain'_cons
+  | x :: y :: l => simp [and_assoc]; intro; exact Chain'_append (l := y :: l)
+
+theorem Chain'.append (hl : Chain' R l) (hlr : ∀ x ∈ l.last', ∀ y ∈ r.head?, R x y) (hr : Chain' R r) : Chain' R (l ++ r) :=
+  Chain'_append.mpr ⟨hl, hlr, hr⟩
+
+end List
+
+inductive BTree (α : Type u)
+  | leaf
+  | node (l : BTree α) (x : α) (r : BTree α)
+
+namespace BTree
+
+variable {α : Type u}
+
+@[simp]
+def toList : BTree α → List α
+  | leaf       => []
+  | node l x r => toList l ++ x :: toList r
+
+@[simp]
+def size : BTree α → Nat
+  | leaf       => 0
+  | node l _ r => size l + size r + 1
+
+@[simp]
+def height : BTree α → Nat
+  | leaf       => 0
+  | node l _ r => max (height l) (height r) + 1
+
+private def toList.impl : BTree α → List α :=
+  toList []
+where
+  toList a
+  | leaf       => a
+  | node l x r => toList (x :: toList a r) l
+
+@[csimp]
+private theorem toList.eq_impl : @toList = @impl := by
+  funext α t
+  suffices ∀ a t, toList t ++ a = impl.toList a t from
+    (List.append_nil .. ▸ this [] t :)
+  intro a t
+  induction t generalizing a with
+  | leaf => rfl
+  | node _ _ _ ihl ihr =>
+    dsimp [toList, impl.toList]
+    rw [← ihr, ← ihl, List.append_assoc]
+    rfl
+
+@[simp]
+def front? : BTree α → Option α
+  | leaf          => none
+  | node leaf x _ => some x
+  | node l    _ _ => front? l
+
+@[simp]
+def back? : BTree α → Option α
+  | leaf          => none
+  | node _ x leaf => some x
+  | node _ _ r    => back? r
+
+theorem head?_toList : (t : BTree α) → t.toList.head? = t.front?
+  | leaf               => rfl
+  | node leaf      _ _ => rfl
+  | node (node ..) _ _ => by simp; rw [← List.head?_append_cons]; exact head?_toList (node ..)
+
+theorem last'_toList : (t : BTree α) → t.toList.last' = t.back?
+  | leaf               => rfl
+  | node _ _ leaf      => by simp
+  | node _ _ (node ..) => by simp; rw [← List.last'_append_cons]; exact last'_toList (node ..)
+
+variable [LT α]
+
+theorem leaf_lt (x : α) : ∀ y ∈ leaf.back?, y < x := λ _ hy => nomatch hy
+theorem leaf_gt (x : α) : ∀ y ∈ leaf.front?, x < y := λ _ hy => nomatch hy
+
+inductive Bst : BTree α → Prop
+  | leaf : Bst leaf
+  | node {l x r} : (∀ y ∈ l.back?, y < x) → (∀ y ∈ r.front?, x < y) → Bst l → Bst r → Bst (node l x r)
+
+theorem Bst_iff_Chain_toList {t : BTree α} : Bst t ↔ t.toList.Chain' LT.lt := by
+  constructor
+  . intro h
+    induction h with
+    | leaf => dsimp!
+    | node hlx hrx _ _ ihl ihr =>
+      dsimp
+      refine .append ihl ?_ <| .cons (head?_toList _ ▸ hrx) ihr
+      simp
+      exact last'_toList _ ▸ hlx
+  . intro h
+    induction t with
+    | leaf => constructor
+    | node _ _ _ ihl ihr =>
+      simp [List.Chain'_append, List.Chain'_cons] at h
+      constructor
+      . exact last'_toList _ ▸ h.2.1
+      . exact head?_toList _ ▸ h.2.2.1
+      . exact ihl h.1
+      . exact ihr h.2.2.2
+
+variable [@DecidableRel α LT.lt]
+
+instance instDecidableBst : (t : BTree α) → Decidable (Bst t)
+  | leaf => isTrue .leaf
+  | node l _ r =>
+    if hlx : _
+    then
+      if hrx : _
+      then
+        match instDecidableBst l with
+        | isTrue hl =>
+          match instDecidableBst r with
+          | isTrue hr => isTrue <| .node hlx hrx hl hr
+          | isFalse hr => isFalse λ | .node _ _ _ hr' => hr hr'
+        | isFalse hl => isFalse λ | .node _ _ hl' _ => hl hl'
+      else isFalse λ | .node _ hrx' _ _ => hrx hrx'
+    else isFalse λ | .node hlx' _ _ _ => hlx hlx'
+
+@[simp]
+def find (y : α) : BTree α → Bool
+  | leaf => false
+  | node l x r => if y < x then find y l else if x < y then find y r else true
+
+def insert (y : α) : BTree α → BTree α
+  | leaf => node leaf y leaf
+  | node l x r => if y < x then node (insert y l) x r else if x < y then node l x (insert y r) else node l x r
+
+theorem insert_lt {t : BTree α} (hyz : y < z) (hlz : ∀ x ∈ t.back?, x < z) : ∀ x ∈ (t.insert y).back?, x < z := by
+  induction t with
+  | leaf => simp [hyz]
+  | node _ _ r _ ihr =>
+    unfold insert
+    split
+    . cases r <;> exact hlz
+    . split
+      . cases r with
+        | leaf => simp [hyz]
+        | node =>
+          specialize ihr hlz
+          unfold insert at ihr ⊢
+          split
+          next h => rw [if_pos h] at ihr; exact ihr
+          next h =>
+            rw [if_neg h] at ihr; split
+            next h => rw [if_pos h] at ihr; exact ihr
+            next h => rw [if_neg h] at ihr; exact ihr
+      . exact hlz
+
+theorem insert_gt {t : BTree α} (hyz : z < y) (hlz : ∀ x ∈ t.front?, z < x) : ∀ x ∈ (t.insert y).front?, z < x := by
+  induction t with
+  | leaf => simp [hyz]
+  | node l _ _ ihl =>
+    unfold insert
+    split
+    . cases l with
+      | leaf => simp [hyz]
+      | node =>
+        specialize ihl hlz
+        unfold insert at ihl ⊢
+        split
+        next h => rw [if_pos h] at ihl; exact ihl
+        next h =>
+          rw [if_neg h] at ihl; split
+          next h => rw [if_pos h] at ihl; exact ihl
+          next h => rw [if_neg h] at ihl; exact ihl
+    . split
+      . cases l <;> exact hlz
+      . exact hlz
+
+theorem insert_Bst {t : BTree α} (h : Bst t) : Bst (t.insert y) := by
+  induction h with
+  | leaf =>
+    refine .node ?_ ?_ .leaf .leaf
+    . simp
+    . simp
+  | node hlx hrx hl hr =>
+    unfold insert
+    split
+    next h => exact .node (insert_lt h hlx) hrx (insert_Bst hl) hr
+    next =>
+      split
+      next h => exact .node hlx (insert_gt h hrx) hl (insert_Bst hr)
+      next => exact .node hlx hrx hl hr
+
+theorem Bst.rotate_left {r : BTree α} : Bst (.node l x (.node c y r)) → Bst (.node (.node l x c) y r)
+  | .node hlx hcyrx hl (.node _   hry     .leaf     hr) => .node (by simp [*]) hry (.node hlx (leaf_gt x) hl .leaf) hr
+  | .node hlx hcyrx hl (.node hcy hry hc@(.node ..) hr) => .node  hcy          hry (.node hlx  hcyrx      hl  hc  ) hr
+
+theorem Bst.rotate_right {r : BTree α} : Bst (.node (.node l x c) y r) → Bst (.node l x (.node c y r))
+  | .node hlxcy hry (.node hlx _   hl     .leaf    ) hr => .node hlx (by simp [*]) hl (.node (leaf_lt y) hry .leaf hr)
+  | .node hlxcy hry (.node hlx hcx hl hc@(.node ..)) hr => .node hlx  hcx          hl (.node  hlxcy      hry  hc   hr)
+
+variable (l r : Nat) in
+inductive Close : Prop
+  | balanced : l = r → Close
+  | left : l = r + 1 → Close
+  | right : l + 1 = r → Close
+
+inductive Avl : BTree α → Prop
+  | leaf : Avl leaf
+  | node : Close l.height r.height → Avl l → Avl r → Avl (node l x r)
+
+def rebalance (l : BTree α) (x : α) (r : BTree α) : BTree α × α × BTree α :=
+  if _ : r.height + 1 < l.height
+  then
+    match l with
+    | node l₁ x₁ r₁ =>
+      if _ : l₁.height < r₁.height
+      then
+        match r₁ with
+        | node l₂ x₂ r₂ => (node l₁ x₁ l₂, x₂, node r₂ x r)
+      else (l₁, x₁, node r₁ x r)
+  else
+    if _ : l.height + 1 < r.height
+    then
+      match r with
+      | node l₁ x₁ r₁ =>
+        if _ : r₁.height < l₁.height
+        then
+          match l₁ with
+          | node l₂ x₂ r₂ => (node l x l₂, x₂, node r₂ x₁ r₁)
+        else (node l x l₁, x₁, r₁)
+    else (l, x, r)
+
+#check Nat.sub_le_sub_left
+
+theorem Close_rebalance {l} {x : α} {r} : let (l', _, r') := rebalance l x r; Close l'.height r'.height := by
+  dsimp
+  unfold rebalance
+  split
+  case' inr =>
+    split
+    case inr h₁ h₂ =>
+      dsimp
+      generalize height l = l at h₁ h₂
+      generalize height r = r at h₁ h₂
+      cases Nat.le_of_not_lt h₁ with
+      | refl => exact .left rfl
+      | step h₁ =>
+      cases Nat.le_of_not_lt h₂ with
+      | refl => exact .right rfl
+      | step h₂ => exact .balanced (Nat.le_antisymm h₁ h₂)
+  . split
+    next l₁ x₁ r₁ _ _ =>
+    split
+    . sorry
+    . dsimp
+      sorry
+  . sorry
+
+variable (y : α) in
+def insertAvl' : BTree α → BTree α × α × BTree α
+  | leaf => (leaf, y, leaf)
+  | node l x r =>
+    if y < x
+    then
+      let (l', x', r') := insertAvl' l
+      rebalance (node l' x' r') x r
+    else
+      if x < y
+      then
+        let (l', x', r') := insertAvl' r
+        rebalance l x (node l' x' r')
+      else (l, x, r)
+
+def insertAvl (y : α) (t : BTree α) : BTree α :=
+  let (l, x, r) := insertAvl' y t
+  node l x r
+
+end BTree
+
+variable (α : Type u) [LT α] in
+def Bst := { t : BTree α // t.Bst }
+
+namespace Bst
+
+variable {α : Type u} [LT α]
+
+def empty : Bst α := ⟨.leaf, .leaf⟩
+
+def singleton (x : α) : Bst α := ⟨.node .leaf x .leaf, .node (BTree.leaf_lt x) (BTree.leaf_gt x) .leaf .leaf⟩
+
+def size (t : Bst α) : Nat := t.val.size
+
+variable [@DecidableRel α LT.lt]
+
+def find (x : α) (t : Bst α) : Bool := t.val.find x
+
+def insert (x : α) (t : Bst α) : Bst α := ⟨t.val.insert x, BTree.insert_Bst t.property⟩
+
+end Bst
+
+def foo : Bst Nat := ⟨.node (.node (.node .leaf 0 .leaf) 2 (.node .leaf 3 .leaf)) 4 (.node (.node .leaf 5 .leaf) 6 (.node .leaf 7 .leaf)), by decide⟩
+#eval foo.1.toList
+
+#eval foo.insert 1 |>.1.toList
+
+#reduce BTree.leaf |>.insertAvl 0 |>.insertAvl 1 |>.insertAvl 2 |>.insertAvl 3 |>.insertAvl 4 |>.insertAvl 5 |>.insertAvl 6 |>.insertAvl 7
+
+/-
+@[simp]
+def Bst' : BTree α → Prop
+  | leaf => True
+  | node l x r => l.lt x ∧ r.gt x ∧ Bst l ∧ Bst r
+
+@[simp]
+example : (t : BTree α) → Bst t ↔ Bst' t
+  | leaf => ⟨λ | .leaf => .intro, λ | .intro => .leaf⟩
+  | node .. => ⟨λ | .node hxl hxr hl hr => ⟨hxl, hxr, hl, hr⟩, λ | ⟨hxl, hxr, hl, hr⟩ => .node hxl hxr hl hr⟩
+-/
