Common/Rel.lean
@@ -1,0 +1,77 @@
+variable {α : Sort u} (r : α → α → Prop)
+
+class Reflexive : Prop where
+  refl : r x x
+
+theorem Reflexive.ofEq {r : α → α → Prop} [Reflexive r] {x y} (h : x = y) : r x y := h ▸ refl
+
+class Symmetric : Prop where
+  symm : r x y → r y x
+
+class Transitive : Prop where
+  trans : r x y → r y z → r x z
+
+class abbrev Equivalence' : Prop := Reflexive r, Symmetric r, Transitive r
+
+inductive ReflexiveTransitiveClosure : α → α → Prop
+  | base : r x y → ReflexiveTransitiveClosure x y
+  | refl : ReflexiveTransitiveClosure x x
+  | trans : ReflexiveTransitiveClosure x y → ReflexiveTransitiveClosure y z → ReflexiveTransitiveClosure x z
+
+instance ReflexiveTransitiveClosure.instReflexive : Reflexive (ReflexiveTransitiveClosure r) := ⟨@refl α r⟩
+instance ReflexiveTransitiveClosure.instTransitive : Transitive (ReflexiveTransitiveClosure r) := ⟨@trans α r⟩
+
+section rec
+
+variable {r} {motive : ∀ x y, ReflexiveTransitiveClosure r x y → Prop}
+  (base : ∀ {x y} h, motive x y (base h))
+  (refl : ∀ {x}, motive x x refl)
+
+def ReflexiveTransitiveClosure.recl
+  (trans : ∀ {x y z} h₁ h₂, motive x y h₁ → motive x z (trans h₁ (.base h₂)))
+: ∀ {x y} h, motive x y h :=
+  @rec α r motive base refl λ {x y z} h₁ h₂ ih₁ _ =>
+    @rec α r (λ y z h₂ => ∀ h₁, motive x y h₁ → motive x z (.trans h₁ h₂))
+      (λ h₂ h₁ => trans h₁ h₂)
+      (λ _ ih₁ => ih₁)
+      (λ h₂ _ r₁ r₂ h₁ ih₁ => r₁ h₁ ih₁ |> r₂ (.trans h₁ h₂))
+    y z h₂ h₁ ih₁
+
+def ReflexiveTransitiveClosure.recr
+  (trans : ∀ {x y z} h₁ h₂, motive y z h₂ → motive x z (trans (.base h₁) h₂))
+: ∀ {x y} h, motive x y h :=
+  @rec α r motive base refl λ {x y z} h₁ h₂ _ =>
+    @rec α r (λ x y h₁ => ∀ h₂, motive y z h₂ → motive x z (.trans h₁ h₂))
+      trans
+      (λ _ ih₂ => ih₂)
+      (λ _ h₁ r₁ r₂ h₂ ih₂ => r₁ (.trans h₁ h₂) <| r₂ h₂ ih₂)
+    x y h₁ h₂
+
+end rec
+
+def ReflexiveTransitiveClosure.lift {β : Sort v} {r s} {f : α → β} (h : ∀ {x y}, r x y → s (f x) (f y)) :
+  ∀ {x y}, ReflexiveTransitiveClosure r x y → ReflexiveTransitiveClosure s (f x) (f y)
+:=
+  @rec α r _
+    (base <| h ·)
+    refl
+    (λ _ _ => trans)
+
+inductive EquivalenceClosure : α → α → Prop
+  | base : r x y → EquivalenceClosure x y
+  | refl : EquivalenceClosure x x
+  | symm : EquivalenceClosure x y → EquivalenceClosure y x
+  | trans : EquivalenceClosure x y → EquivalenceClosure y z → EquivalenceClosure x z
+
+instance EquivalenceClosure.instReflexive : Reflexive (EquivalenceClosure r) := ⟨@refl α r⟩
+instance EquivalenceClosure.instSymmetric : Symmetric (EquivalenceClosure r) := ⟨@symm α r⟩
+instance EquivalenceClosure.instTransitive : Transitive (EquivalenceClosure r) := ⟨@trans α r⟩
+
+def EquivalenceClosure.lift {β : Sort v} {r s} {f : α → β} (h : ∀ {x y}, r x y → s (f x) (f y)) :
+  ∀ {x y}, EquivalenceClosure r x y → EquivalenceClosure s (f x) (f y)
+:=
+  @rec α r _
+    (base <| h ·)
+    refl
+    (λ _ => symm)
+    (λ _ _ => trans)
