rec/Rec/Util.lean
@@ -118,13 +118,168 @@ theorem map_erase cmp x t : map f (erase cmp x t) = erase cmp x (map f t) := by
 theorem WellFormed.mapWff (w : WellFormed cmp n) : WellFormed cmp (map f n) := by
   induction w with
   | leafWff => exact leafWff
-  | insertWff _ h ih => exact h ▸ insertWff ih (map_insert ..)
-  | eraseWff _ h ih => exact h ▸ eraseWff ih (map_erase ..)
+  | insertWff _ h ih => cases h; exact insertWff ih (map_insert ..)
+  | eraseWff _ h ih => cases h; exact eraseWff ih (map_erase ..)
+
+/-
+@[simp]
+theorem ofMap_leaf : map f t = leaf ↔ t = leaf := by
+  cases t <;> simp [map]
+
+@[simp]
+theorem ofMap_node  : map f t = node c l k v r ↔ ∃ l' v' r', t = node c l' k v' r' ∧ map f l' = l ∧ f k v' = v ∧ map f r' = r := by
+  constructor
+  . intro h
+    cases t <;> cases h
+    exact ⟨_, _, _, rfl, rfl, rfl, rfl⟩
+  . intro ⟨_, _, _, _⟩
+    simp [map, *]
+
+macro "destruct" : tactic =>
+  `(tactic| ((repeat first | cases ‹Exists ..› | cases ‹And ..›); subst_vars))
+
+section
+
+local syntax "by_match " term " with" ("| " term)* : term
+macro_rules
+  | `(by_match $t with $[| $p]*) =>
+    let q := p
+    `(by match $t:term with $[| $p => intro h; simp [balance1] at h; destruct; exact ⟨$q, _, _, rfl, rfl, rfl, rfl⟩]*)
+
+theorem ofMap_balance1 : map f t = balance1 l k v r → ∃ l' v' r', t = balance1 l' k v' r' ∧ map f l' = l ∧ f k v' = v ∧ map f r' = r :=
+  by_match l with
+  | leaf
+  | node .red leaf _ _ leaf
+  | node .red leaf _ _ (node .red ..)
+  | node .red leaf _ _ (node .black ..)
+  | node .red (node .red ..) _ _ leaf
+  | node .red (node .red ..) _ _ (node .red ..)
+  | node .red (node .red ..) _ _ (node .black ..)
+  | node .red (node .black ..) _ _ leaf
+  | node .red (node .black ..) _ _ (node .red ..)
+  | node .red (node .black ..) _ _ (node .black ..)
+  | node .black ..
+
+end
+
+section
+
+local syntax "by_match " term " with" ("| " term)* : term
+macro_rules
+  | `(by_match $t with $[| $p]*) =>
+    let q := p
+    `(by match $t:term with $[| $p => intro h; simp [balance2] at h; destruct; exact ⟨_, _, $q, rfl, rfl, rfl, rfl⟩]*)
+
+theorem ofMap_balance2 : map f t = balance2 l k v r → ∃ l' v' r', t = balance2 l' k v' r' ∧ map f l' = l ∧ f k v' = v ∧ map f r' = r :=
+  by_match r with
+  | leaf
+  | node .red leaf _ _ leaf
+  | node .red leaf _ _ (node .red ..)
+  | node .red leaf _ _ (node .black ..)
+  | node .red (node .red ..) _ _ leaf
+  | node .red (node .red ..) _ _ (node .red ..)
+  | node .red (node .red ..) _ _ (node .black ..)
+  | node .red (node .black ..) _ _ leaf
+  | node .red (node .black ..) _ _ (node .red ..)
+  | node .red (node .black ..) _ _ (node .black ..)
+  | node .black ..
+
+end
+
+theorem ofMap_ins (heq : ∀ {x y}, cmp x y = .eq → x = y) : map f t = ins cmp t' k v → ∃ t'' v', t = ins cmp t'' k v' := by
+  unfold ins
+  split
+  . simp; intro; destruct; exact ⟨leaf, _, rfl⟩
+  . split
+    . simp; intro; destruct; have := ofMap_ins heq ‹_›; destruct; exact ⟨node .red .., _, by dsimp; rw [‹cmp .. = _›]⟩
+    . simp; intro; destruct; have := ofMap_ins heq ‹_›; destruct; exact ⟨node .red .., _, by dsimp; rw [‹cmp .. = _›]⟩
+    . simp; intro; destruct; exact ⟨node .red .., _, by dsimp; rw [‹cmp .. = _›]; exact heq ‹cmp .. = _› ▸ ‹_›⟩
+  . split
+    . intro h; have := ofMap_balance1 f h; clear h; destruct; have := ofMap_ins heq ‹_›; destruct; exact ⟨node .black .., _, by dsimp; rw [‹cmp .. = _›]⟩
+    . intro h; have := ofMap_balance2 f h; clear h; destruct; have := ofMap_ins heq ‹_›; destruct; exact ⟨node .black .., _, by dsimp; rw [‹cmp .. = _›]⟩
+    . simp; intro; destruct; exact ⟨node .black .., _, by dsimp; rw [‹cmp .. = _›]; exact heq ‹cmp .. = _› ▸ ‹_›⟩
+
+theorem ofMap_setBlack : map f t = setBlack t' → ∃ t'', t = setBlack t'' := by
+  cases t'
+  . simp [setBlack]; intro; destruct; exact ⟨leaf, rfl⟩
+  . simp [setBlack]; intro; destruct; exact ⟨node ‹_› .., rfl⟩
+
+theorem ofMap_insert (heq : ∀ {x y}, cmp x y = .eq → x = y) (h : map f t = insert cmp t' k v) : ∃ t'' v', t = insert cmp t'' k v' := by
+  unfold insert at h ⊢
+  split at h
+  . have := ofMap_setBlack f h; destruct; rw [map_setBlack] at h; sorry
+  . have := ofMap_ins f heq h; destruct; exact ⟨‹_›, _, by dsimp; sorry⟩
+
+theorem ins_ne_leaf : ins cmp t k v ≠ leaf := by
+  unfold ins
+  split
+  . simp
+  . split <;> simp
+  . split
+    . unfold balance1
+      split <;> simp
+    . unfold balance2
+      split <;> simp
+    . simp
+
+theorem insert_ne_leaf : insert cmp t k v ≠ leaf := by
+  unfold insert
+  split
+  . unfold setBlack
+    split
+    . simp
+    . exact ins_ne_leaf
+  . exact ins_ne_leaf
+
+theorem ofMap_insert (h : map f t = insert cmp t' k v) : ∃ t'' v', t = insert cmp t'' k v' := by
+  cases t <;> cases t' <;> dsimp [map, insert, isRed] at h ⊢
+  . simp at h; cases ins_ne_leaf h.symm
+  . sorry
+  . sorry
+  . sorry
+
+theorem WellFormed.ofMapWff (w : WellFormed cmp (map f n)) : WellFormed cmp n := by
+  generalize hn' : map f n = n' at w
+  induction w generalizing n with
+  | leafWff => cases n; exact leafWff; cases hn'
+  | insertWff _ h ih => cases h; cases n; dsimp [map] at hn'; cases insert_ne_leaf hn'.symm; have := ofMap_insert f sorry hn'; destruct; rename_i h; rw [h, map_insert] at hn'; exact insertWff (ih sorry) ‹_›
+  | eraseWff _ h ih => cases h; sorry -- exact h ▸ eraseWff ih (map_erase ..)
+
+variable {α : Type u} {β γ : α → Type u} {m : Type u → Type v} [Applicative m] (f : (a : α) → β a → m (γ a)) in
+def mapM' : (t : RBNode α β) → m { t' : RBNode α γ // t.map (λ _ _ => PUnit.unit) = t'.map (λ _ _ => PUnit.unit) }
+  | leaf => pure ⟨leaf, rfl⟩
+  | node color lchild key val rchild =>
+    (λ ⟨lchild', _⟩ val' ⟨rchild', _⟩ => ⟨node color lchild' key val' rchild', by unfold map; congr⟩) <$> mapM' lchild <*> f key val <*> mapM' rchild
+  -/
 
 end Lean.RBNode
 
 def Lean.RBMap.map (f : α → β → γ) : RBMap α β cmp → RBMap α γ cmp
   | ⟨t, w⟩ => ⟨.map f t, .mapWff f w⟩
 
-def Lean.RBMap.mapM [Monad m] (f : α → β → m γ) : RBMap α β cmp → m (RBMap α γ cmp)
-  | ⟨t, w⟩ => return ⟨← t.mapM f, sorry⟩
+def Lean.RBMap.mapM [Applicative m]  (f : α → β → m γ) : RBMap α β cmp → m (RBMap α γ cmp)
+  | ⟨t, w⟩ =>
+    --(λ ⟨t', h⟩ => ⟨t', .ofMapWff (λ _ _ => PUnit.unit) <| h ▸ .mapWff _ w⟩) <$> t.mapM' f
+    (⟨·, sorry⟩) <$> t.mapM f
+
+/-
+attribute [local simp]
+  Functor.map SeqLeft.seqLeft SeqRight.seqRight Seq.seq bind
+  EStateM.map EStateM.seqRight EStateM.bind
+
+instance : LawfulMonad (EStateM ε σ) where
+  map_const := rfl
+  id_map _ := by funext _; simp; split <;> simp [*]
+  seqLeft_eq _ _ := by funext _; simp; split <;> rfl
+  seqRight_eq _ _ := by funext _; simp; split; split <;> assumption; rfl
+  pure_seq _ _ := rfl
+  bind_pure_comp _ _ := rfl
+  bind_map _ _ := rfl
+  pure_bind _ _ := rfl
+  bind_assoc _ _ _ := by
+    funext _; simp; split
+    . split at *; simp [*]; contradiction
+    . split at *; simp [*]; injections; simp [*]
+
+instance : LawfulMonad (EIO ε) := instLawfulMonadEStateMInstMonadEStateM
+-/
